Some housekeeping changes to do with action graphs.
1. Actions can take lists of writes.  What they do with those writes
   is unspecified; some later apply_action function has the
   responsibility to apply the contents of the type to whatever is
   being updated.

2. The "iter" field is renamed to "ident" and the "expr" field is
   renamed to "data".

This is all looking forward to supporting graphs with nodes that are
themselves graphs.

Proofs have all been made to work again.

hol/PseudoCPropsScript.sml
@@ -302,13 +302,13 @@ val updf_def = Define`
 
 val apply_action_def = Define`
   apply_action a m_opt =
-    case a.write of
-        NONE => m_opt
-      | SOME w =>
+    case a.writes of
+        [] => m_opt
+      | (w::_) =>
         do
           m <- m_opt;
           vs <- SOME(MAP (lookupRW m) a.reads);
-          value <- SOME (a.expr vs);
+          value <- SOME (a.data vs);
           updf w value m
         od
 `;
@@ -354,7 +354,7 @@ val updf_preserves_FDOMs = store_thm(
 val apply_action_preserves_FDOMs = store_thm(
   "apply_action_preserves_FDOMs",
   ``apply_action a (SOME m) = SOME m' ⇒ FDOM m' = FDOM m``,
-  simp[apply_action_def] >> Cases_on `a.write` >> simp[] >>
+  simp[apply_action_def] >> Cases_on `a.writes` >> simp[] >>
   metis_tac[updf_preserves_FDOMs]);
 
 val updf_preserves_array_presence_length_back = store_thm(
@@ -384,8 +384,8 @@ val updf_preserves_array_presence_length_forward = store_thm(
 val m_t = ``m:memory``
 val m'_t = ``m':memory``
 
-val nontouching_updfs_read_after_write = store_thm(
-  "nontouching_updfs_read_after_write",
+val nontouching_updfs_read_after_writes = store_thm(
+  "nontouching_updfs_read_after_writes",
   ``updf w value m = SOME m' ∧ w ≠ rd ⇒ lookupRW m' rd = lookupRW m rd``,
   `(∃a i. w = Array a i) ∨ ∃s. w = Variable s` by (Cases_on `w` >> simp[]) >>
   `(∃b j. rd = Array b j) ∨ ∃t. rd = Variable t` by (Cases_on `rd` >> simp[]) >>
@@ -420,11 +420,11 @@ val nontouching_updfs_read_after_write = store_thm(
 
 val nontouching_updfs_expreval = store_thm(
   "nontouching_updfs_expreval",
-  ``¬(touches a1 a2) ∧ a2.write = SOME w ∧ updf w value m = SOME m' ⇒
+  ``¬(touches a1 a2) ∧ a2.writes = w::rest ∧ updf w value m = SOME m' ⇒
     MAP (lookupRW m') a1.reads = MAP (lookupRW m) a1.reads``,
   simp[MAP_EQ_f] >> strip_tac >> qx_gen_tac `r` >> strip_tac >>
-  `r ≠ w` by metis_tac[touches_def] >>
-  metis_tac[nontouching_updfs_read_after_write]);
+  `r ≠ w` by metis_tac[touches_def, MEM] >>
+  metis_tac[nontouching_updfs_read_after_writes]);
 
 val FLOOKUP_memory_cases = prove(
   ``!x: value option.
@@ -511,7 +511,7 @@ fun eqNONE_tac (g as (asl,w)) = let
     disj2_tac >> disj2_tac >> disj1_tac >> AP_TERM_TAC >>
     simp[MAP_EQ_f] >> rpt strip_tac >>
     qunabbrev_tac [QUOTE other_name] >> fs[] >>
-    metis_tac[nontouching_updfs_read_after_write, touches_def]
+    metis_tac[nontouching_updfs_read_after_writes, touches_def]
   val expr_case =
     rpt disj2_tac >>
     qpat_assum `XX = Array ZZ:value`
@@ -519,7 +519,7 @@ fun eqNONE_tac (g as (asl,w)) = let
                 REWRITE_TAC [SYM th]) >> AP_TERM_TAC >>
     simp[MAP_EQ_f] >> rpt strip_tac >>
     qunabbrev_tac [QUOTE other_name] >> fs[] >>
-    metis_tac[nontouching_updfs_read_after_write, touches_def]
+    metis_tac[nontouching_updfs_read_after_writes, touches_def]
   val vararray_case =
     qunabbrev_tac [QUOTE other_name] >> fs[] >>
     qpat_assum `mm : memory ' vv = Array eee` assume_tac >>
@@ -631,43 +631,47 @@ val success_case =
   rpt (first_x_assum (kall_tac o assert (is_forall o concl))) >>
   map_every qunabbrev_tac [`A1U`, `A2U`] >> fs[] >>
   qabbrev_tac `
-    ae = λa:(value,actionRW,α)action m. a.expr (MAP (lookupRW m) a.reads)
+    ae = λa:(value list -> value,actionRW,α)action m.
+             a.data (MAP (lookupRW m) a.reads)
   ` >> fs[] >>
   ae_equate_tac "a1" >> ae_equate_tac "a2" >> fs[] >>
-  metis_tac[updf_writes_commute, touches_def]
+  metis_tac[updf_writes_commute]
 
 
 val apply_action_commutes = store_thm(
   "apply_action_commutes",
-  ``¬(a1:(value,actionRW,α)action ∼ₜ a2:(value,actionRW,α)action) ⇒
-    (apply_action a2 (apply_action a1 m) =
-     apply_action a1 (apply_action a2 m))``,
+  ``a1:(value list -> value,actionRW,α)action ≁ₜ
+    a2:(value list -> value,actionRW,α)action ⇒
+    apply_action a2 (apply_action a1 m) = apply_action a1 (apply_action a2 m)``,
   strip_tac >>
   `m = NONE ∨ ∃gm. m = SOME gm`
      by metis_tac[optionTheory.option_CASES, pair_CASES] >>
   simp[apply_action_def, lift_OPTION_BIND, combinTheory.o_ABS_R,
        o_UNCURRY_R, C_UNCURRY_L,
        combinTheory.C_ABS_L] >>
-  `a1.write = NONE ∨ ∃w1. a1.write = SOME w1`
-    by (Cases_on `a1.write` >> simp[]) >>
-  `a2.write = NONE ∨ ∃w2. a2.write = SOME w2`
-    by (Cases_on `a2.write` >> simp[]) >>
+  `a1.writes = [] ∨ ∃w1 t1. a1.writes = w1::t1`
+    by (Cases_on `a1.writes` >> simp[]) >>
+  `a2.writes = [] ∨ ∃w2 t2. a2.writes = w2::t2`
+    by (Cases_on `a2.writes` >> simp[]) >>
   simp[] >>
   qabbrev_tac `
-    A1U = λm. updf w1 (a1.expr (MAP (lookupRW m) a1.reads)) m` >>
+    A1U = λm. updf w1 (a1.data (MAP (lookupRW m) a1.reads)) m` >>
   qabbrev_tac `
-    A2U = λm. updf w2 (a2.expr (MAP (lookupRW m) a2.reads)) m` >>
+    A2U = λm. updf w2 (a2.data (MAP (lookupRW m) a2.reads)) m` >>
   simp[] >>
   `(∀m m'. A1U m = SOME m' ⇒ FDOM m' = FDOM m) ∧
    (∀m m'. A2U m = SOME m' ⇒ FDOM m' = FDOM m)`
      by (simp[Abbr`A1U`, Abbr`A2U`] >> metis_tac[updf_preserves_FDOMs]) >>
+  `(∀rd. MEM rd a1.reads ⇒ rd ≠ w2) ∧ (∀rd. MEM rd a2.reads ⇒ rd ≠ w1) ∧
+   w1 ≠ w2`
+    by metis_tac[touches_def, MEM] >>
   rpt (findOptionCases >> simp[]) >> fs[] >>
   TRY (eqNONE_tac >> NO_TAC) >>
   success_case)
 
 val commutes_lemma = prove(
   ``∀a1 a2 s.
-      ¬(a1 ∼ₜ a2) ∧ a1.iter ≠ a2.iter ⇒
+      ¬(a1 ∼ₜ a2) ∧ a1.ident ≠ a2.ident ⇒
       apply_action a2 (apply_action a1 s) =
       apply_action a1 (apply_action a2 s)``,
   simp[apply_action_commutes]);
@@ -759,27 +763,27 @@ val expr_reads_def = tDefine "expr_reads" `
 
 val readAction_def = Define`
   readAction i m e = <| reads := expr_reads m e;
-                      write := NONE;
-                      expr := ARB : value list -> value;
-                      iter := i |>
+                      writes := [];
+                      data := ARB : value list -> value;
+                      ident := i |>
 `;
 
-val readAction_iter = store_thm(
-  "readAction_iter[simp]",
-  ``(readAction i m e).iter = i``,
+val readAction_ident = store_thm(
+  "readAction_ident[simp]",
+  ``(readAction i m e).ident = i``,
   simp[readAction_def]);
 
 val domreadAction_def = Define`
   domreadAction i m (D lo hi) =
     <| reads := expr_reads m lo ++ expr_reads m hi;
-       write := NONE;
-       expr := ARB : value list -> value;
-       iter := i |>
+       writes := [];
+       data := ARB : value list -> value;
+       ident := i |>
 `;
 
-val domreadAction_iter = store_thm(
-  "domreadAction_iter[simp]",
-  ``(domreadAction i m d).iter = i``,
+val domreadAction_ident = store_thm(
+  "domreadAction_ident[simp]",
+  ``(domreadAction i m d).ident = i``,
   Cases_on `d` >> simp[domreadAction_def]);
 
 val dvread_def = Define`
@@ -790,14 +794,14 @@ val dvread_def = Define`
 
 val dvreadAction_def = Define`
   dvreadAction i m ds = <| reads := FLAT (MAP (dvread m) ds);
-                           write := NONE;
-                           expr := ARB : value list -> value;
-                           iter := i |>
+                           writes := [];
+                           data := ARB : value list -> value;
+                           ident := i |>
 `
 
-val dvreadAction_iter = store_thm(
-  "dvreadAction_iter[simp]",
-  ``(dvreadAction i m ds).iter = i``,
+val dvreadAction_ident = store_thm(
+  "dvreadAction_ident[simp]",
+  ``(dvreadAction i m ds).ident = i``,
   simp[dvreadAction_def]);
 
 val apply_dvreadAction = store_thm(
@@ -862,10 +866,10 @@ val graphOf_def = tDefine "graphOf" `
         rds <- getReads m0 ds;
         a0 <- SOME (readAction i0 m0 i_e);
         a1 <- SOME (dvreadAction (stackInc i0) m0 ds);
-        a <- SOME <| write := SOME(Array aname i);
+        a <- SOME <| writes := [Array aname i];
                      reads := rds;
-                     expr := mergeReads ds opn;
-                     iter := stackInc (stackInc i0) |> ;
+                     data := mergeReads ds opn;
+                     ident := stackInc (stackInc i0) |> ;
         rvs <- OPT_SEQUENCE (MAP (evalDexpr m0) ds);
         m' <- upd_array m0 aname i (opn rvs);
         SOME(stackInc (stackInc (stackInc i0)), m', a0 ⊕ (a1 ⊕ (a ⊕ emptyG)))
@@ -875,10 +879,10 @@ val graphOf_def = tDefine "graphOf" `
      do
        m' <- updf (Variable vnm) (evalexpr m0 e) m0;
        SOME(stackInc i0, m',
-            <| write := SOME (Variable vnm);
+            <| writes := [Variable vnm];
                reads := expr_reads m0 e;
-               expr := K (evalexpr m0 e);
-               iter := i0 |> ⊕ emptyG)
+               data := K (evalexpr m0 e);
+               ident := i0 |> ⊕ emptyG)
      od) ∧
 
   (graphOf i0 m0 Abort = NONE) ∧
@@ -956,21 +960,21 @@ val OPTION_IGNORE_BIND_EQUALS_OPTION = store_thm(
       (?x'. x = SOME x') /\ (y = SOME z))``,
   Cases_on `x` THEN SIMP_TAC (srw_ss()) []);
 
-val iterations_FOLDR_merge_graph = store_thm(
-  "iterations_FOLDR_merge_graph",
-  ``i ∈ iterations (FOLDR merge_graph g0 glist) ⇔
-    i ∈ iterations g0 ∨ ∃g. MEM g glist ∧ i ∈ iterations g``,
+val idents_FOLDR_merge_graph = store_thm(
+  "idents_FOLDR_merge_graph",
+  ``i ∈ idents (FOLDR merge_graph g0 glist) ⇔
+    i ∈ idents g0 ∨ ∃g. MEM g glist ∧ i ∈ idents g``,
   Induct_on `glist` >> simp[] >> metis_tac[]);
 
 val SNOC_11 = prove(
   ``INJ (λi. i ++ [x]) s UNIV``,
   simp[INJ_THM]);
 
-val iterations_pushG = store_thm(
-  "iterations_pushG",
-  ``i ∈ iterations (pushG n g) ⇔
-    ∃i0. i0 ∈ iterations g ∧ i = i0 ++ [n]``,
-  simp[pushG_def, SNOC_11, iterations_imap] >> metis_tac[]);
+val idents_pushG = store_thm(
+  "idents_pushG",
+  ``i ∈ idents (pushG n g) ⇔
+    ∃i0. i0 ∈ idents g ∧ i = i0 ++ [n]``,
+  simp[pushG_def, SNOC_11, idents_imap] >> metis_tac[]);
 
 val ilistLE_NIL = store_thm(
   "ilistLE_NIL[simp]",
@@ -1061,12 +1065,12 @@ val stackInc_TAKE_lemma = prove(
   simp[stackInc_def] >> Induct_on `l1` >> simp[] >> Cases_on `l2` >>
   simp[] >> Cases_on `l1` >> simp[]);
 
-val graphOf_iterations_apart = store_thm(
-  "graphOf_iterations_apart",
+val graphOf_idents_apart = store_thm(
+  "graphOf_idents_apart",
   ``∀i0 m0 c i m g.
        graphOf i0 m0 c = SOME(i,m,g) ∧ i0 ≠ [] ⇒
        i0 ≤ i ∧ LENGTH i = LENGTH i0 ∧ FRONT i = FRONT i0 ∧
-       ∀j. j ∈ iterations g ⇒ i0 ≤ j ∧ j < i ∧
+       ∀j. j ∈ idents g ⇒ i0 ≤ j ∧ j < i ∧
            LENGTH i0 ≤ LENGTH j ∧
            TAKE (LENGTH i0 - 1) j = FRONT i0``,
   ho_match_mp_tac (theorem "graphOf_ind") >> rpt conj_tac
@@ -1113,8 +1117,8 @@ val graphOf_iterations_apart = store_thm(
       metis_tac[ilistLTE_trans, ilistLE_LTEQ])
   >- ((* Par *)
       map_every qx_gen_tac [`i0`, `m0`, `c`] >> strip_tac >>
-      simp[Once graphOf_def, PULL_EXISTS, iterations_FOLDR_merge_graph,
-           PULL_EXISTS, iterations_pushG, ilistLT_stackInc,
+      simp[Once graphOf_def, PULL_EXISTS, idents_FOLDR_merge_graph,
+           PULL_EXISTS, idents_pushG, ilistLT_stackInc,
            OPT_SEQUENCE_EQ_SOME, MEM_MAPi, MEM_MAP,
            EXISTS_PROD, combinTheory.o_ABS_R] >>
       qabbrev_tac `GG = λn. graphOf (i0 ++ [n;0]) m0 (EL n c)` >> simp[] >>
@@ -1160,7 +1164,7 @@ val graphOf_iterations_apart = store_thm(
 
 val pcg_eval_merge_graph = store_thm(
   "pcg_eval_merge_graph",
-  ``(∀a. a ∈ g1 ⇒ a.iter ∉ iterations g2) ⇒
+  ``(∀a. a ∈ g1 ⇒ a.ident ∉ idents g2) ⇒
     pcg_eval (merge_graph g1 g2) m_opt = pcg_eval g2 (pcg_eval g1 m_opt)``,
   map_every qid_spec_tac [`m_opt`, `g2`, `g1`] >>
   ho_match_mp_tac graph_ind >> simp[pcg_eval_thm] >>
@@ -1202,13 +1206,13 @@ val add_action_id' = add_action_id |> EQ_IMP_RULE |> #2
 val pcg_eval_readAction = store_thm(
   "pcg_eval_readAction[simp]",
   ``pcg_eval (readAction i m e ⊕ g) mo = pcg_eval g mo``,
-  Cases_on `i ∈ iterations g` >> simp[pcg_eval_thm, add_action_id'] >>
+  Cases_on `i ∈ idents g` >> simp[pcg_eval_thm, add_action_id'] >>
   simp[readAction_def, apply_action_def]);
 
 val pcg_eval_domreadAction = store_thm(
   "pcg_eval_domreadAction[simp]",
   ``pcg_eval (domreadAction i m d ⊕ g) mo = pcg_eval g mo``,
-  Cases_on `i ∈ iterations g` >> simp[pcg_eval_thm, add_action_id'] >>
+  Cases_on `i ∈ idents g` >> simp[pcg_eval_thm, add_action_id'] >>
   Cases_on `d` >> simp[domreadAction_def, apply_action_def]);
 
 val graphOf_pcg_eval = store_thm(
@@ -1230,11 +1234,11 @@ val graphOf_pcg_eval = store_thm(
       simp[pcg_eval_thm, PULL_EXISTS, FORALL_PROD] >>
       fs[] >> map_every qx_gen_tac [`i`, `m`, `i'`, `m'`, `g1`, `g2`] >>
       strip_tac >>
-      `i0 ≤ i' ∧ (∀j. j ∈ iterations g1 ⇒ j < i') ∧ i' ≠ [] ∧
-       (∀j. j ∈ iterations g2 ⇒ i' ≤ j)`
-         by metis_tac[graphOf_iterations_apart, ilistLE_NIL] >>
-      `∀a. a ∈ g1 ⇒ a.iter ∉ iterations g2`
-        by (fs[iterations_thm, PULL_EXISTS] >>
+      `i0 ≤ i' ∧ (∀j. j ∈ idents g1 ⇒ j < i') ∧ i' ≠ [] ∧
+       (∀j. j ∈ idents g2 ⇒ i' ≤ j)`
+         by metis_tac[graphOf_idents_apart, ilistLE_NIL] >>
+      `∀a. a ∈ g1 ⇒ a.ident ∉ idents g2`
+        by (fs[idents_thm, PULL_EXISTS] >>
             metis_tac[ilistLTE_trans, ilistLE_REFL]) >>
       simp[pcg_eval_merge_graph] >> fs[])
   >- ((* parloop *)
@@ -1273,44 +1277,44 @@ val INJ_UNION_DOMAIN = store_thm(
 
 val add_postactionID = store_thm(
   "add_postactionID",
-  ``a.iter ∈ iterations g ⇒ add_postaction a g = g``,
+  ``a.ident ∈ idents g ⇒ add_postaction a g = g``,
   simp[graph_equality, add_postaction_edges]);
 
 val imap_add_postaction = store_thm(
   "imap_add_postaction",
-  ``INJ f (a.iter INSERT iterations g) UNIV ⇒
+  ``INJ f (a.ident INSERT idents g) UNIV ⇒
     imap f (add_postaction a g) =
-        add_postaction (a with iter updated_by f) (imap f g)``,
+        add_postaction (a with ident updated_by f) (imap f g)``,
   map_every qid_spec_tac [`a`, `g`] >> ho_match_mp_tac graph_ind >>
   simp[imap_add_action] >> map_every qx_gen_tac [`a`, `g`] >>
   strip_tac >> qx_gen_tac `b` >> strip_tac >>
-  `INJ f (a.iter INSERT iterations g) UNIV` by fs[INJ_INSERT] >>
-  `INJ f (b.iter INSERT iterations g) UNIV` by fs[INJ_INSERT] >>
-  Cases_on `b.iter = a.iter`
-  >- simp[add_postactionID, iterations_imap] >>
-  `f a.iter ≠ f b.iter` by fs[INJ_THM] >>
+  `INJ f (a.ident INSERT idents g) UNIV` by fs[INJ_INSERT] >>
+  `INJ f (b.ident INSERT idents g) UNIV` by fs[INJ_INSERT] >>
+  Cases_on `b.ident = a.ident`
+  >- simp[add_postactionID, idents_imap] >>
+  `f a.ident ≠ f b.ident` by fs[INJ_THM] >>
   fs[imap_add_action, add_action_add_postaction_ASSOC, INSERT_COMM]);
 
 val imap_merge_graph = store_thm(
   "imap_merge_graph",
-  ``INJ f (iterations g1 ∪ iterations g2) UNIV ∧
-    DISJOINT (iterations g1) (iterations g2) ⇒
+  ``INJ f (idents g1 ∪ idents g2) UNIV ∧
+    DISJOINT (idents g1) (idents g2) ⇒
     imap f (merge_graph g1 g2) = merge_graph (imap f g1) (imap f g2)``,
   map_every qid_spec_tac [`g1`, `g2`] >> ho_match_mp_tac graph_ind >>
   simp[merge_graph_thm] >> rpt strip_tac >>
   fs[INSERT_UNION_EQ, ONCE_REWRITE_RULE [UNION_COMM] INSERT_UNION_EQ] >>
-  `DISJOINT (iterations g1) (iterations g2) ∧
-   DISJOINT (a.iter INSERT iterations g1) (iterations g2)`
+  `DISJOINT (idents g1) (idents g2) ∧
+   DISJOINT (a.ident INSERT idents g1) (idents g2)`
     by (fs[DISJOINT_DEF, EXTENSION] >> metis_tac[]) >>
-  `INJ f (a.iter INSERT iterations g1) UNIV ∧
-   INJ f (a.iter INSERT iterations g2) UNIV ∧
-   INJ f (iterations g1) UNIV ∧ INJ f (iterations g2) UNIV`
+  `INJ f (a.ident INSERT idents g1) UNIV ∧
+   INJ f (a.ident INSERT idents g2) UNIV ∧
+   INJ f (idents g1) UNIV ∧ INJ f (idents g2) UNIV`
     by (fs[INJ_UNION_DOMAIN, INJ_INSERT] >> fs[INJ_THM] >>
         metis_tac[]) >>
-  `∀j. j ∈ iterations g1 ∨ j ∈ iterations g2 ⇒ (f a.iter ≠ f j)`
+  `∀j. j ∈ idents g1 ∨ j ∈ idents g2 ⇒ (f a.ident ≠ f j)`
     by (rpt strip_tac >> fs[INJ_INSERT, DISJOINT_DEF, EXTENSION] >>
         metis_tac[]) >>
-  csimp[imap_add_action, merge_graph_thm, iterations_imap,
+  csimp[imap_add_action, merge_graph_thm, idents_imap,
         imap_add_postaction, INSERT_UNION_EQ,
         ONCE_REWRITE_RULE [UNION_COMM] INSERT_UNION_EQ]);
 
@@ -1319,12 +1323,12 @@ val INJ_CONG = store_thm(
   ``(∀x. x ∈ s ⇒ f x = g x) ⇒ (INJ f s t ⇔ INJ g s t)``,
   simp[INJ_THM]);
 
-val iterations_FOLDRi_merge = store_thm(
-  "iterations_FOLDRi_merge",
+val idents_FOLDRi_merge = store_thm(
+  "idents_FOLDRi_merge",
   ``∀g.
-      iterations (FOLDRi (λn c. merge_graph (g n c)) a l) =
-        BIGUNION (IMAGE (λi. iterations (g i (EL i l))) (count (LENGTH l))) ∪
-        iterations a``,
+      idents (FOLDRi (λn c. merge_graph (g n c)) a l) =
+        BIGUNION (IMAGE (λi. idents (g i (EL i l))) (count (LENGTH l))) ∪
+        idents a``,
   Induct_on `l` >> simp[combinTheory.o_ABS_L] >>
   dsimp[Once EXTENSION, LT_SUC] >> metis_tac[]);
 
@@ -1338,12 +1342,12 @@ val imap_FOLDRi_merge = store_thm(
   "imap_FOLDRi_merge",
   ``∀f g.
       (∀i j. i < j ∧ j < LENGTH l ⇒
-        DISJOINT (iterations (g i (EL i l)))
-                 (iterations (g j (EL j l)))) ∧
+        DISJOINT (idents (g i (EL i l)))
+                 (idents (g j (EL j l)))) ∧
       (∀i. i < LENGTH l ⇒
-           DISJOINT (iterations (g i (EL i l))) (iterations G)) ∧
-      INJ f (iterations G ∪
-             iterations (FOLDRi (λn c. merge_graph (g n c)) G l))
+           DISJOINT (idents (g i (EL i l))) (idents G)) ∧
+      INJ f (idents G ∪
+             idents (FOLDRi (λn c. merge_graph (g n c)) G l))
             UNIV
      ⇒
       imap f (FOLDRi (λn c. merge_graph (g n c)) G l) =
@@ -1360,7 +1364,7 @@ val imap_FOLDRi_merge = store_thm(
   `imap f (merge_graph (g 0 h) AG) = merge_graph (imap f (g 0 h)) (imap f AG)`
     by (match_mp_tac imap_merge_graph >> conj_tac
         >- (first_x_assum match_mp_tac >> simp[SUBSET_DEF]) >>
-        dsimp[Abbr`AG`, iterations_FOLDRi_merge] >>
+        dsimp[Abbr`AG`, idents_FOLDRi_merge] >>
         metis_tac[DISJOINT_SYM]) >>
   simp[combinTheory.o_DEF]);
 
@@ -1394,7 +1398,7 @@ val graphOf_starting_id_irrelevant = store_thm(
         i0' ≠ [] ⇒
         ∃f.
           graphOf i0' m0 c0 = SOME(f i, m, imap f g) ∧
-          i0' = f i0 ∧ INJ f (i INSERT iterations g) UNIV``,
+          i0' = f i0 ∧ INJ f (i INSERT idents g) UNIV``,
   ho_match_mp_tac (theorem "graphOf_ind") >> rpt conj_tac >>
   map_every qx_gen_tac [`i0`, `m0`]
   >- (qx_gen_tac `gd` >> rpt gen_tac >> strip_tac >>
@@ -1408,20 +1412,20 @@ val graphOf_starting_id_irrelevant = store_thm(
       disch_then (qx_choose_then `f` strip_assume_tac) >> simp[] >>
       qabbrev_tac `ff = λj. if j = i0 then i0' else f j` >>
       qexists_tac `ff` >> simp[] >>
-      `stackInc i0 ≤ i ∧ ∀j. j ∈ iterations g ⇒ stackInc i0 ≤ j`
-        by metis_tac[graphOf_iterations_apart, stackInc_EQ_NIL] >>
+      `stackInc i0 ≤ i ∧ ∀j. j ∈ idents g ⇒ stackInc i0 ≤ j`
+        by metis_tac[graphOf_idents_apart, stackInc_EQ_NIL] >>
       `i0 < stackInc i0` by metis_tac[ilistLT_stackInc] >>
       `i0 < i ∧ i0 ≠ i` by metis_tac[ilistLE_REFL, ilistLTE_trans] >>
-      `i0 ∉ iterations g` by metis_tac[ilistLTE_trans, ilistLE_REFL] >>
+      `i0 ∉ idents g` by metis_tac[ilistLTE_trans, ilistLE_REFL] >>
       `ff i0 = i0' ∧ ff i = f i` by simp[Abbr`ff`] >> simp[] >>
-      `∀j. j ∈ iterations g ⇒ ff j = f j` by (simp[Abbr`ff`] >> metis_tac[]) >>
-      `INJ ff (i0 INSERT iterations g) UNIV`
+      `∀j. j ∈ idents g ⇒ ff j = f j` by (simp[Abbr`ff`] >> metis_tac[]) >>
+      `INJ ff (i0 INSERT idents g) UNIV`
         by (simp[INJ_INSERT] >> simp[Cong INJ_CONG] >>
             asm_simp_tac (srw_ss() ++ CONJ_ss ++ ETA_ss) [] >>
             fs[INJ_INSERT] >> qx_gen_tac `y` >> strip_tac >>
-            `f y ∈ iterations (imap f g)` by simp[iterations_imap] >>
+            `f y ∈ idents (imap f g)` by simp[idents_imap] >>
             `stackInc i0' ≤ f y`
-              by metis_tac[graphOf_iterations_apart, stackInc_EQ_NIL] >>
+              by metis_tac[graphOf_idents_apart, stackInc_EQ_NIL] >>
             `i0' < stackInc i0'` by metis_tac[ilistLT_stackInc] >>
             metis_tac[ilistLTE_trans, ilistLE_REFL]) >>
       simp[imap_add_action] >> simp[Cong imap_CONG] >>
@@ -1429,7 +1433,7 @@ val graphOf_starting_id_irrelevant = store_thm(
       asm_simp_tac (srw_ss() ++ CONJ_ss ++ DNF_ss) [] >>
       qx_gen_tac `y` >> fs[INJ_INSERT] >> Cases_on `y = i0` >> simp[] >>
       `stackInc i0' ≤ f i`
-        by metis_tac[graphOf_iterations_apart, stackInc_EQ_NIL] >>
+        by metis_tac[graphOf_idents_apart, stackInc_EQ_NIL] >>
       `i0' < stackInc i0'` by metis_tac[ilistLT_stackInc] >>
       metis_tac[ilistLTE_trans, ilistLE_REFL])
   >- (rpt gen_tac >> strip_tac >> ONCE_REWRITE_TAC [graphOf_def] >>
@@ -1441,26 +1445,26 @@ val graphOf_starting_id_irrelevant = store_thm(
       qabbrev_tac `ff = λk. if k = i0 then j else f k` >> qexists_tac `ff` >>
       `i0 < stackInc i0 ∧ j < stackInc j ∧ stackInc i0 ≠ [] ∧ stackInc j ≠ []`
         by simp[] >>
-      `(∀k. k ∈ iterations g ⇒ stackInc i0 ≤ k ∧ i0 < k) ∧ stackInc i0 ≤ i ∧
+      `(∀k. k ∈ idents g ⇒ stackInc i0 ≤ k ∧ i0 < k) ∧ stackInc i0 ≤ i ∧
        i0 < i`
-        by metis_tac[graphOf_iterations_apart, ilistLTE_trans, ilistLE_REFL]>>
-      `i0 ∉ iterations g ∧ i0 ≠ i` by metis_tac[ilistLE_REFL] >>
+        by metis_tac[graphOf_idents_apart, ilistLTE_trans, ilistLE_REFL]>>
+      `i0 ∉ idents g ∧ i0 ≠ i` by metis_tac[ilistLE_REFL] >>
       `ff i0 = j ∧ ff i = f i` by simp[Abbr`ff`] >>
-      `∀k. k ∈ iterations g ⇒ ff k = f k` by (simp[Abbr`ff`] >> metis_tac[]) >>
+      `∀k. k ∈ idents g ⇒ ff k = f k` by (simp[Abbr`ff`] >> metis_tac[]) >>
       simp[] >>
-      `INJ ff (i0 INSERT iterations g) UNIV`
+      `INJ ff (i0 INSERT idents g) UNIV`
         by (fs[INJ_INSERT, Cong INJ_CONG] >> csimp[] >> qx_gen_tac `y` >>
             strip_tac >> full_simp_tac (srw_ss() ++ ETA_ss) [] >>
-            `f y ∈ iterations (imap f g)` by simp[iterations_imap] >>
+            `f y ∈ idents (imap f g)` by simp[idents_imap] >>
             `stackInc (f y) ≤ f y`
-              by metis_tac[graphOf_iterations_apart, stackInc_EQ_NIL] >>
+              by metis_tac[graphOf_idents_apart, stackInc_EQ_NIL] >>
             metis_tac[ilistLT_stackInc, stackInc_EQ_NIL,
                       ilistLTE_trans, ilistLE_REFL]) >>
       simp[imap_add_action] >> simp[Cong imap_CONG] >>
       Cases_on `d` >> simp[domreadAction_def] >> simp[Once INJ_INSERT] >>
       dsimp[] >> csimp[] >> fs[INJ_INSERT] >>
       `stackInc j ≤ f i`
-        by metis_tac[graphOf_iterations_apart, stackInc_EQ_NIL] >>
+        by metis_tac[graphOf_idents_apart, stackInc_EQ_NIL] >>
       metis_tac[ilistLT_stackInc, ilistLTE_trans, ilistLE_REFL])
   >- ((* seq *)
       qx_gen_tac `cs` >> Cases_on `cs` >> simp[]
@@ -1472,7 +1476,7 @@ val graphOf_starting_id_irrelevant = store_thm(
       map_every qx_gen_tac [`i`, `m`, `i0'`, `m0'`, `g1`, `g2`] >>
       strip_tac >> qx_gen_tac `j` >> strip_tac >>
       `∃f1. graphOf j m0 h = SOME(f1 i0',m0',imap f1 g1) ∧ j = f1 i0 ∧
-            INJ f1 (i0' INSERT iterations g1) UNIV`
+            INJ f1 (i0' INSERT idents g1) UNIV`
         by metis_tac[] >> simp[] >>
       Q.UNDISCH_THEN `graphOf i0 m0 h = SOME(i0',m0',g1)`
         (fn th => first_x_assum
@@ -1480,56 +1484,56 @@ val graphOf_starting_id_irrelevant = store_thm(
                                  assume_tac th)) >>
       simp[] >>
       first_x_assum (kall_tac o assert(is_forall o concl)) >>
-      `i0' ≠ [] ∧ i0 ≤ i0' ∧ i0' ≤ i ∧ (∀k. k ∈ iterations g1 ⇒ k < i0') ∧
-       ∀k. k ∈ iterations g2 ⇒ i0' ≤ k`
-        by metis_tac[graphOf_iterations_apart, ilistLE_NIL] >>
+      `i0' ≠ [] ∧ i0 ≤ i0' ∧ i0' ≤ i ∧ (∀k. k ∈ idents g1 ⇒ k < i0') ∧
+       ∀k. k ∈ idents g2 ⇒ i0' ≤ k`
+        by metis_tac[graphOf_idents_apart, ilistLE_NIL] >>
       simp[] >>
-      `DISJOINT (iterations g1) (iterations g2)`
+      `DISJOINT (idents g1) (idents g2)`
         by (simp[DISJOINT_DEF, EXTENSION] >>
             metis_tac[ilistLTE_trans, ilistLE_REFL]) >>
       disch_then (qspec_then `f1 i0'` mp_tac) >> simp[] >>
-      `f1 i0' ≠ [] ∧ (∀k. k ∈ iterations (imap f1 g1) ⇒ k < f1 i0')`
-        by metis_tac[graphOf_iterations_apart, ilistLE_NIL] >>
+      `f1 i0' ≠ [] ∧ (∀k. k ∈ idents (imap f1 g1) ⇒ k < f1 i0')`
+        by metis_tac[graphOf_idents_apart, ilistLE_NIL] >>
       simp[] >> disch_then (qx_choose_then `f2` strip_assume_tac) >>
       simp[] >>
-      `∀k. k ∈ iterations (imap f2 g2) ⇒ f1 i0' ≤ k`
-        by metis_tac[graphOf_iterations_apart] >>
-      `INJ f1 (iterations g1) UNIV ∧ INJ f2 (iterations g2) UNIV`
+      `∀k. k ∈ idents (imap f2 g2) ⇒ f1 i0' ≤ k`
+        by metis_tac[graphOf_idents_apart] >>
+      `INJ f1 (idents g1) UNIV ∧ INJ f2 (idents g2) UNIV`
         by fs[INJ_INSERT] >>
       qabbrev_tac `
-        ff = λk. if k ∈ iterations g2 ∨ k = i then f2 k else f1 k` >>
+        ff = λk. if k ∈ idents g2 ∨ k = i then f2 k else f1 k` >>
       qexists_tac `ff` >>
       `f2 i = ff i` by simp[Abbr`ff`] >> simp[] >>
       `f1 i0 = ff i0`
         by (rw[Abbr`ff`] >> metis_tac[ilistLE_antisym]) >> simp[] >>
-      `i ∉ iterations g1` by metis_tac[ilistLTE_trans, ilistLE_REFL] >>
-      `(∀k. k ∈ iterations g1 ⇒ ff k = f1 k) ∧
-       (∀k. k ∈ iterations g2 ⇒ ff k = f2 k)`
+      `i ∉ idents g1` by metis_tac[ilistLTE_trans, ilistLE_REFL] >>
+      `(∀k. k ∈ idents g1 ⇒ ff k = f1 k) ∧
+       (∀k. k ∈ idents g2 ⇒ ff k = f2 k)`
         by (simp[Abbr`ff`] >> qx_gen_tac `k` >> strip_tac >>
-            `k ∉ iterations g2 ∧ k ≠ i`
+            `k ∉ idents g2 ∧ k ≠ i`
               by (fs[DISJOINT_DEF, EXTENSION] >> metis_tac[]) >>
             simp[]) >>
-      `INJ ff (iterations g1 ∪ iterations g2) UNIV`
+      `INJ ff (idents g1 ∪ idents g2) UNIV`
         by (simp[INJ_UNION_DOMAIN] >>
-            `INJ ff (iterations g1) UNIV ∧ INJ ff (iterations g2) UNIV`
+            `INJ ff (idents g1) UNIV ∧ INJ ff (idents g2) UNIV`
               by full_simp_tac (srw_ss() ++ ETA_ss)
                    [Cong INJ_CONG] >>
-            `iterations g1 DIFF iterations g2 = iterations g1 ∧
-             iterations g2 DIFF iterations g1 = iterations g2`
+            `idents g1 DIFF idents g2 = idents g1 ∧
+             idents g2 DIFF idents g1 = idents g2`
               by (fs[DISJOINT_DEF, EXTENSION] >> metis_tac[]) >>
             simp[Cong (REWRITE_RULE [GSYM AND_IMP_INTRO] IMAGE_CONG)] >>
             CONV_TAC (DEPTH_CONV ETA_CONV) >>
-            fs[iterations_imap, PULL_EXISTS] >>
+            fs[idents_imap, PULL_EXISTS] >>
             simp[DISJOINT_DEF, EXTENSION] >>
             metis_tac[ilistLTE_trans, ilistLE_REFL]) >>
       simp[imap_merge_graph, Cong imap_CONG] >>
       simp[INJ_INSERT] >> dsimp[] >> reverse conj_tac
-      >- (`∀k. k ∈ iterations (imap f2 g2) ⇒ k < ff i`
-            by metis_tac[graphOf_iterations_apart] >> pop_assum mp_tac >>
-          dsimp[iterations_imap] >> csimp[] >> metis_tac[ilistLE_REFL]) >>
+      >- (`∀k. k ∈ idents (imap f2 g2) ⇒ k < ff i`
+            by metis_tac[graphOf_idents_apart] >> pop_assum mp_tac >>
+          dsimp[idents_imap] >> csimp[] >> metis_tac[ilistLE_REFL]) >>
       csimp[] >>
-      `f2 i0' ≤ f2 i` by metis_tac[graphOf_iterations_apart] >>
-      fs[iterations_imap, PULL_EXISTS] >>
+      `f2 i0' ≤ f2 i` by metis_tac[graphOf_idents_apart] >>
+      fs[idents_imap, PULL_EXISTS] >>
       metis_tac[ilistLE_REFL, ilistLTE_trans])
   >- ((* parloop *)
       map_every qx_gen_tac [`vnm`, `d`, `body`] >>
@@ -1542,26 +1546,26 @@ val graphOf_starting_id_irrelevant = store_thm(
       qabbrev_tac `ff = λk. if k = i0 then j else f k` >> qexists_tac `ff` >>
       `i0 < stackInc i0 ∧ j < stackInc j ∧ stackInc i0 ≠ [] ∧ stackInc j ≠ []`
         by simp[] >>
-      `(∀k. k ∈ iterations g ⇒ stackInc i0 ≤ k ∧ i0 < k) ∧ stackInc i0 ≤ i ∧
+      `(∀k. k ∈ idents g ⇒ stackInc i0 ≤ k ∧ i0 < k) ∧ stackInc i0 ≤ i ∧
        i0 < i`
-        by metis_tac[graphOf_iterations_apart, ilistLTE_trans, ilistLE_REFL]>>
-      `i0 ∉ iterations g ∧ i0 ≠ i` by metis_tac[ilistLE_REFL] >>
+        by metis_tac[graphOf_idents_apart, ilistLTE_trans, ilistLE_REFL]>>
+      `i0 ∉ idents g ∧ i0 ≠ i` by metis_tac[ilistLE_REFL] >>
       `ff i0 = j ∧ ff i = f i` by simp[Abbr`ff`] >>
-      `∀k. k ∈ iterations g ⇒ ff k = f k` by (simp[Abbr`ff`] >> metis_tac[]) >>
+      `∀k. k ∈ idents g ⇒ ff k = f k` by (simp[Abbr`ff`] >> metis_tac[]) >>
       simp[] >>
-      `INJ ff (i0 INSERT iterations g) UNIV`
+      `INJ ff (i0 INSERT idents g) UNIV`
         by (fs[INJ_INSERT, Cong INJ_CONG] >> csimp[] >> qx_gen_tac `y` >>
             strip_tac >> full_simp_tac (srw_ss() ++ ETA_ss) [] >>
-            `f y ∈ iterations (imap f g)` by simp[iterations_imap] >>
+            `f y ∈ idents (imap f g)` by simp[idents_imap] >>
             `stackInc (f y) ≤ f y`
-              by metis_tac[graphOf_iterations_apart, stackInc_EQ_NIL] >>
+              by metis_tac[graphOf_idents_apart, stackInc_EQ_NIL] >>
             metis_tac[ilistLT_stackInc, stackInc_EQ_NIL,
                       ilistLTE_trans, ilistLE_REFL]) >>
       simp[imap_add_action] >> simp[Cong imap_CONG] >>
       Cases_on `d` >> simp[domreadAction_def] >> simp[Once INJ_INSERT] >>
       dsimp[] >> csimp[] >> fs[INJ_INSERT] >>
       `stackInc j ≤ f i`
-        by metis_tac[graphOf_iterations_apart, stackInc_EQ_NIL] >>
+        by metis_tac[graphOf_idents_apart, stackInc_EQ_NIL] >>
       metis_tac[ilistLT_stackInc, ilistLTE_trans, ilistLE_REFL])
   >- ((* Par *)
       qx_gen_tac `cs` >> strip_tac >>
@@ -1596,7 +1600,7 @@ val graphOf_starting_id_irrelevant = store_thm(
                   else if i = stackInc i0 then stackInc i0'
                   else ff (EL (LENGTH i0) i) i` >>
       qexists_tac `fff` >>
-      `∀n. n < LENGTH cs ⇒ INJ (ff n) (iterations (gfg n)) UNIV`
+      `∀n. n < LENGTH cs ⇒ INJ (ff n) (idents (gfg n)) UNIV`
         by metis_tac[INJ_INSERT]>>
       `∀n. n < LENGTH cs ⇒ ∃z. GG i0' n (EL n cs) = SOME z`
         by simp[Abbr`GG`] >> simp[] >>
@@ -1611,12 +1615,12 @@ val graphOf_starting_id_irrelevant = store_thm(
         by simp[LIST_EQ_REWRITE] >>
       fs[] >> ntac 2 (pop_assum kall_tac) >>
       fs[FOLDR_MAPi, combinTheory.o_ABS_R] >>
-      `∀n j. n < LENGTH cs ∧ j ∈ iterations (imap (ff n) (gfg n)) ⇒
+      `∀n j. n < LENGTH cs ∧ j ∈ idents (imap (ff n) (gfg n)) ⇒
              i0' ++ [n;0] ≤ j ∧
              TAKE (LENGTH (i0' ++ [n;0]) - 1) j = FRONT (i0' ++ [n;0])`
         by (rpt gen_tac >> strip_tac >> res_tac >>
             `i0' ++ [n;0] ≠ []` by simp[] >>
-            metis_tac[graphOf_iterations_apart]) >>
+            metis_tac[graphOf_idents_apart]) >>
       fs[FRONT_APPEND] >>
       `imap fff (FOLDRi (λn c. merge_graph (gfg n)) emptyG cs) =
        FOLDRi (λn c. merge_graph (imap fff (gfg n))) (imap fff emptyG) cs`
@@ -1627,20 +1631,20 @@ val graphOf_starting_id_irrelevant = store_thm(
             conj_tac
             >- (simp[DISJOINT_DEF, EXTENSION] >>
                 map_every qx_gen_tac [`i`, `j`] >> strip_tac >>
-                qx_gen_tac `it` >> Cases_on `it ∈ iterations (gfg i)` >>
+                qx_gen_tac `it` >> Cases_on `it ∈ idents (gfg i)` >>
                 simp[] >>
                 `i < LENGTH cs` by decide_tac >> strip_tac >>
                 `TAKE (LENGTH (i0 ++ [i;0]) - 1) it = i0 ++ [i] ∧
                  TAKE (LENGTH (i0 ++ [j;0]) - 1) it = i0 ++ [j]`
-                  by metis_tac[graphOf_iterations_apart] >>
+                  by metis_tac[graphOf_idents_apart] >>
                 fs[]) >>
-            dsimp[iterations_FOLDRi_merge, INJ_THM] >>
+            dsimp[idents_FOLDRi_merge, INJ_THM] >>
             map_every qx_gen_tac [`it1`, `it2`, `i`, `j`] >> strip_tac >>
             `TAKE (LENGTH (i0 ++ [i;0]) - 1) it1 = i0 ++ [i] ∧
              TAKE (LENGTH (i0 ++ [j;0]) - 1) it2 = i0 ++ [j] ∧
              LENGTH (i0 ++ [i;0]) ≤ LENGTH it1 ∧
              LENGTH (i0 ++ [j;0]) ≤ LENGTH it2`
-                by metis_tac[graphOf_iterations_apart] >>
+                by metis_tac[graphOf_idents_apart] >>
             lfs[] >>
             `EL (LENGTH i0) it1 = EL (LENGTH i0) (i0 ++ [i]) ∧
              EL (LENGTH i0) it2 = EL (LENGTH i0) (i0 ++ [j])`
@@ -1653,16 +1657,16 @@ val graphOf_starting_id_irrelevant = store_thm(
               by (rpt strip_tac >> lfs[]) >> simp[] >>
             reverse (Cases_on `i = j`)
             >- (`it1 ≠ it2` by (strip_tac >> fs[]) >> simp[] >>
-                `ff i it1 ∈ iterations (imap (ff i) (gfg i)) ∧
-                 ff j it2 ∈ iterations (imap (ff j) (gfg j))`
-                  by simp[iterations_imap] >>
+                `ff i it1 ∈ idents (imap (ff i) (gfg i)) ∧
+                 ff j it2 ∈ idents (imap (ff j) (gfg j))`
+                  by simp[idents_imap] >>
                 `∀i. i < LENGTH cs ⇒ ff i (i0 ++ [i; 0]) ≠ []`
                   by metis_tac[APPEND_eq_NIL, NOT_CONS_NIL] >>
                 `TAKE (LENGTH (i0' ++ [i;0]) - 1) (ff i it1) =
                  FRONT (i0' ++ [i;0]) ∧
                  TAKE (LENGTH (i0' ++ [j;0]) - 1) (ff j it2) =
                  FRONT (i0' ++ [j;0])`
-                  by metis_tac[graphOf_iterations_apart] >>
+                  by metis_tac[graphOf_idents_apart] >>
                 fs[FRONT_APPEND] >>
                 strip_tac >> fs[]) >>
             pop_assum SUBST_ALL_TAC >> fs[INJ_THM]) >>
@@ -1673,7 +1677,7 @@ val graphOf_starting_id_irrelevant = store_thm(
               simp[] >> qx_gen_tac `it` >> strip_tac >>
               `LENGTH (i0 ++ [i;0]) ≤ LENGTH it ∧
                TAKE (LENGTH (i0 ++ [i;0]) - 1) it = FRONT (i0 ++ [i;0])`
-                by metis_tac[graphOf_iterations_apart, APPEND_eq_NIL,
+                by metis_tac[graphOf_idents_apart, APPEND_eq_NIL,
                              NOT_CONS_NIL] >>
               `it ≠ i0 ∧ it ≠ stackInc i0` by (rpt strip_tac >> lfs[]) >>
               simp[] >> lfs[FRONT_APPEND] >>
@@ -1686,13 +1690,13 @@ val graphOf_starting_id_irrelevant = store_thm(
         >- simp[Abbr`fff`]
         >- ((* injectivity of fff *)
             asm_simp_tac (srw_ss() ++ ETA_ss ++ DNF_ss)
-                         [INJ_INSERT, iterations_FOLDRi_merge] >>
-            `∀i n. i ∈ iterations (gfg n) ∧ n < LENGTH cs ⇒
+                         [INJ_INSERT, idents_FOLDRi_merge] >>
+            `∀i n. i ∈ idents (gfg n) ∧ n < LENGTH cs ⇒
                    LENGTH (i0 ++ [n;0]) ≤ LENGTH i ∧
                    TAKE (LENGTH (i0 ++ [n;0]) - 1) i = FRONT (i0 ++ [n;0])`
               by metis_tac[APPEND_eq_NIL, NOT_CONS_NIL,
-                           graphOf_iterations_apart] >>
-            `∀i n. i ∈ iterations (gfg n) ∧ n < LENGTH cs ⇒
+                           graphOf_idents_apart] >>
+            `∀i n. i ∈ idents (gfg n) ∧ n < LENGTH cs ⇒
                    EL (LENGTH i0) i = n`
               by (rpt strip_tac >> lfs[FRONT_APPEND] >> res_tac >>
                   `EL (LENGTH i0) i =
@@ -1700,7 +1704,7 @@ val graphOf_starting_id_irrelevant = store_thm(
                     by simp[EL_TAKE] >> simp[EL_APPEND2]) >>
             reverse conj_tac
             >- (map_every qx_gen_tac [`y`, `n`] >> strip_tac >>
-                qpat_assum `y ∈ iterations (gfg n)`
+                qpat_assum `y ∈ idents (gfg n)`
                   (fn i => qpat_assum `n < LENGTH cs`
                   (fn l => rpt (first_x_assum
                                   (strip_assume_tac o
@@ -1710,10 +1714,10 @@ val graphOf_starting_id_irrelevant = store_thm(
                 simp[Abbr`fff`] >> lfs[FRONT_APPEND] >>
                 `y ≠ i0 ∧ y ≠ stackInc i0` by (rpt strip_tac >> lfs[]) >>
                 simp[] >>
-                `ff n y ∈ iterations (imap (ff n) (gfg n))`
-                  by simp[iterations_imap] >>
+                `ff n y ∈ idents (imap (ff n) (gfg n))`
+                  by simp[idents_imap] >>
                 `LENGTH (i0' ++ [n; 0]) ≤ LENGTH (ff n y)`
-                  by metis_tac[graphOf_iterations_apart, NOT_CONS_NIL,
+                  by metis_tac[graphOf_idents_apart, NOT_CONS_NIL,
                                APPEND_eq_NIL] >>
                 fs[] >> strip_tac >> `ff n y = stackInc i0'` by simp[] >>
                 lfs[]) >>
@@ -1732,14 +1736,14 @@ val graphOf_starting_id_irrelevant = store_thm(
             Cases_on `i = j`
             >- (pop_assum SUBST_ALL_TAC >> metis_tac[INJ_DEF]) >>
             `it1 ≠ it2` by (strip_tac >> fs[]) >> simp[] >>
-            `ff i it1 ∈ iterations (imap (ff i) (gfg i)) ∧
-             ff j it2 ∈ iterations (imap (ff j) (gfg j))`
-              by simp[iterations_imap] >>
+            `ff i it1 ∈ idents (imap (ff i) (gfg i)) ∧
+             ff j it2 ∈ idents (imap (ff j) (gfg j))`
+              by simp[idents_imap] >>
             qpat_assum `imap fff ggg = XXX` kall_tac >>
             qpat_assum `∀i. i < LENGTH cs ⇒ imap fff ggg = g'g'g'` kall_tac >>
             `TAKE (LENGTH (i0' ++ [i;0]) - 1) (ff i it1) = FRONT (i0' ++ [i;0]) ∧
              TAKE (LENGTH (i0' ++ [j;0]) - 1) (ff j it2) = FRONT (i0' ++ [j;0])`
-              by metis_tac[graphOf_iterations_apart, NOT_CONS_NIL,
+              by metis_tac[graphOf_idents_apart, NOT_CONS_NIL,
                            APPEND_eq_NIL] >> lfs[FRONT_APPEND] >>
             strip_tac >> lfs[]))
   >- ((* assign *)
@@ -1829,7 +1833,7 @@ val pcg_eval_NONE = store_thm(
   "pcg_eval_NONE[simp]",
   ``∀g. pcg_eval g NONE = NONE``,
   ho_match_mp_tac graph_ind >> simp[pcg_eval_thm, apply_action_def] >>
-  rpt gen_tac >> Cases_on `a.write` >> simp[]);
+  rpt gen_tac >> Cases_on `a.writes` >> simp[]);
 
 val expr_ind' = store_thm(
   "expr_ind'",
@@ -1849,16 +1853,19 @@ val apply_action_expr_eval_commutes = store_thm(
        readAction j m0 e ≁ₜ a ∧ apply_action a (SOME m0) = SOME m ⇒
        evalexpr m e = evalexpr m0 e ∧ readAction j m e = readAction j m0 e``,
   simp[readAction_def, touches_def, apply_action_def] >> gen_tac >>
-  `a.write = NONE ∨ ∃w. a.write = SOME w` by (Cases_on `a.write` >> simp[]) >>
-  simp[] >> pop_assum kall_tac >> gen_tac >>
-  map_every qspec_tac [(`a.expr`, `expr`), (`a.reads`, `rds`), (`w`, `w`)] >>
-  qid_spec_tac `e` >> ho_match_mp_tac expr_ind' >>
+  `a.writes = [] ∨ ∃w t. a.writes = w::t` by (Cases_on `a.writes` >> simp[]) >>
+  simp[] >>
+  REWRITE_TAC [DECIDE ``p \/ q <=> ~p ==> q``] >> simp[DISJ_IMP_THM, FORALL_AND_THM] >>
+  pop_assum kall_tac >> map_every qx_gen_tac [`e`, `m0`, `m`] >> strip_tac >>
+  first_x_assum (kall_tac o assert (is_forall o concl)) >> rpt (pop_assum mp_tac) >>
+  map_every qspec_tac [(`a.data`, `expr`), (`a.reads`, `rds`)] >>
+  map_every qid_spec_tac [`m0`, `m`, `e`] >> ho_match_mp_tac expr_ind' >>
   simp[evalexpr_def, expr_reads_def] >> rpt conj_tac
   >- (simp[MEM_FLAT, MEM_MAP] >> rpt strip_tac >>
       AP_TERM_TAC >> simp[MAP_EQ_f] >> metis_tac[])
   >- (map_every qx_gen_tac [`anm`, `e`] >> strip_tac >>
-      map_every qx_gen_tac [`w`, `rds`, `expr`, `m0`, `m`] >>
-      strip_tac >>
+      map_every qx_gen_tac [`m`, `m0`, `rds`, `expr`] >>
+      rpt strip_tac >>
       `¬MEM w (expr_reads m0 e)` by (Cases_on `evalexpr m0 e` >> fs[]) >>
       `evalexpr m e = evalexpr m0 e ∧ expr_reads m e = expr_reads m0 e`
         by metis_tac[] >>
@@ -1911,7 +1918,6 @@ val apply_action_dvalues_commutes = store_thm(
     by metis_tac[apply_action_expr_eval_commutes, touches_SYM] >>
   simp[dvalues_def] >> fs[readAction_def, action_component_equality]);
 
-
 val successful_action_diamond = store_thm(
   "successful_action_diamond",
   ``a1 ≁ₜ a2 ∧ apply_action a1 (SOME m0) = SOME m1 ∧
@@ -1919,10 +1925,10 @@ val successful_action_diamond = store_thm(
     ∃m. apply_action a1 (SOME m2) = SOME m ∧
         apply_action a2 (SOME m1) = SOME m``,
   simp[apply_action_def, SimpL ``$==>``] >>
-  `a1.write = NONE ∨ ∃w1. a1.write = SOME w1`
-    by (Cases_on `a1.write` >> simp[]) >>
-  `a2.write = NONE ∨ ∃w2. a2.write = SOME w2`
-    by (Cases_on `a2.write` >> simp[]) >> simp[apply_action_def]
+  `a1.writes = [] ∨ ∃w1 t1. a1.writes = w1::t1`
+    by (Cases_on `a1.writes` >> simp[]) >>
+  `a2.writes = [] ∨ ∃w2 t2. a2.writes = w2::t2`
+    by (Cases_on `a2.writes` >> simp[]) >> simp[apply_action_def]
   >- (rw[] >> simp[]) >> strip_tac >> simp[] >> rw[] >>
   `MAP (lookupRW m2) a1.reads = MAP (lookupRW m0) a1.reads ∧
    MAP (lookupRW m1) a2.reads = MAP (lookupRW m0) a2.reads`
@@ -1930,9 +1936,7 @@ val successful_action_diamond = store_thm(
   simp[] >>
   qmatch_rename_tac
     `∃m. updf w1 v1 m2 = SOME m ∧ updf w2 v2 m1 = SOME m` [] >>
-  fs[touches_def] >>
-  map_every (fn q => Q.UNDISCH_THEN q assume_tac)
-    [`a1.write = SOME w1`, `a2.write = SOME w2`] >> fs[] >>
+  fs[touches_def] >> `w1 ≠ w2` by metis_tac[MEM] >>
   metis_tac[successful_updf_diamond]);
 
 val pcg_eval_apply_action_diamond = store_thm(
@@ -1956,41 +1960,71 @@ val pcg_eval_apply_action_diamond = store_thm(
 val IN_FOLDRi_merge_graph = store_thm(
   "IN_FOLDRi_merge_graph",
   ``(∀i. i < LENGTH list ⇒
-         DISJOINT (iterations (f i (EL i list))) (iterations acc)) ∧
+         DISJOINT (idents (f i (EL i list))) (idents acc)) ∧
     (∀i j. i < j ∧ j < LENGTH list ⇒
-           DISJOINT (iterations (f i (EL i list)))
-                    (iterations (f j (EL j list)))) ⇒
+           DISJOINT (idents (f i (EL i list)))
+                    (idents (f j (EL j list)))) ⇒
     (a ∈ FOLDRi (λn c. merge_graph (f n c)) acc list ⇔
      a ∈ acc ∨ ∃i. i < LENGTH list ∧ a ∈ f i (EL i list))``,
   qid_spec_tac `f` >>
   Induct_on `list` >> dsimp[combinTheory.o_ABS_L, LT_SUC] >>
   rw[EQ_IMP_THM] >> simp[]
   >- metis_tac[]
-  >- (`a.iter ∈ iterations acc` by simp[iterations_thm] >>
+  >- (`a.ident ∈ idents acc` by simp[idents_thm] >>
       fs[DISJOINT_DEF, EXTENSION] >> metis_tac[])
-  >- (`a.iter ∉ iterations (f 0 h)` suffices_by metis_tac[] >>
-      `a.iter ∈ iterations (f (SUC n0) (EL n0 list))` by simp[iterations_thm] >>
+  >- (`a.ident ∉ idents (f 0 h)` suffices_by metis_tac[] >>
+      `a.ident ∈ idents (f (SUC n0) (EL n0 list))` by simp[idents_thm] >>
       fs[DISJOINT_DEF, EXTENSION] >> metis_tac[]))
+
+val mkWFA_def = Define`
+  mkWFA a =
+    case a.writes of
+        [] => a
+      | h::t => <| reads := a.reads ;
+                   writes := [h] ;
+                   data := a.data;
+                   ident := a.ident |>
+`;
+
+val touches_mkWFA = store_thm(
+  "touches_mkWFA",
+  ``mkWFA a ∼ₜ b ⇒ a ∼ₜ b``,
+  simp[touches_def, mkWFA_def] >> Cases_on `a.writes` >> simp[] >>
+  metis_tac[]);
+
+val apply_action_mkWFA = store_thm(
+  "apply_action_mkWFA[simp]",
+  ``apply_action (mkWFA a) m_opt = apply_action a m_opt``,
+  simp[apply_action_def, mkWFA_def] >> Cases_on `m_opt` >> simp[] >>
+  Cases_on `a.writes` >> simp[]);
 
 val apply_action_dvreadAction_commutes = store_thm(
   "apply_action_dvreadAction_commutes",
   ``a ≁ₜ dvreadAction i m0 ds ∧ apply_action a (SOME m0) = SOME m ∧
     getReads m0 ds = SOME rds ∧
-    (IS_SOME a.write ⇒ ¬MEM (THE a.write) rds)
+    (a.writes ≠ [] ⇒ ¬MEM (HD a.writes) rds)
    ⇒
     dvreadAction i m ds = dvreadAction i m0 ds ∧
     getReads m ds = getReads m0 ds ∧
     MAP (evalDexpr m) ds = MAP (evalDexpr m0) ds``,
   simp[dvreadAction_def, touches_def, MEM_FLAT, MEM_MAP, PULL_FORALL,
        GSYM IMP_DISJ_THM] >>
-  `a.write = NONE ∨ ∃w. a.write = SOME w` by (Cases_on `a.write` >> simp[]) >>
+  `a.writes = [] ∨ ∃w t. a.writes = w::t` by (Cases_on `a.writes` >> simp[]) >>
   simp[FORALL_AND_THM, GSYM LEFT_FORALL_OR_THM, PULL_EXISTS,
        GSYM RIGHT_FORALL_OR_THM] >- csimp[apply_action_def] >>
+  simp[DISJ_IMP_THM, FORALL_AND_THM] >>
   Cases_on `apply_action a (SOME m0) = SOME m` >> simp[] >>
+  `apply_action (mkWFA a) (SOME m0) = SOME m` by simp[] >>
+  `(mkWFA a).writes = [w]` by simp[mkWFA_def] >> qabbrev_tac `b = mkWFA a` >>
+  Q.RM_ABBREV_TAC `b` >> ntac 2 (pop_assum mp_tac) >>
+  rpt (pop_assum kall_tac) >> ntac 2 strip_tac >> strip_tac >>
+  first_x_assum
+    (kall_tac o assert (equal 2 o length o #1 o strip_forall o concl)) >>
+  ntac 3 (pop_assum mp_tac) >>
   qid_spec_tac `rds` >> Induct_on `ds` >>
   simp[getReads_def] >> Cases >> simp[getReads_def, dvread_def, evalDexpr_def]
-  >- (simp[dvread_def, DISJ_IMP_THM, FORALL_AND_THM] >> ntac 2 strip_tac >>
-      `readAction i m0 e ≁ₜ a` by simp[readAction_def, touches_def] >>
+  >- (simp[dvread_def, DISJ_IMP_THM, FORALL_AND_THM] >> ntac 4 strip_tac >>
+      `readAction i m0 e ≁ₜ b` by (simp[readAction_def, touches_def]) >>
       `readAction i m e = readAction i m0 e ∧ evalexpr m e = evalexpr m0 e`
         by metis_tac[apply_action_expr_eval_commutes] >>
       fs[readAction_def] >> BasicProvers.VAR_EQ_TAC >> fs[] >>
@@ -1999,18 +2033,23 @@ val apply_action_dvreadAction_commutes = store_thm(
       `evalexpr m0 (ISub anm e) = lookup_array m0 anm i ∧
        evalexpr m (ISub anm e) = lookup_array m anm i`
         by simp[evalexpr_def] >>
-      `a ≁ₜ readAction jj m0 (ISub anm e)`
+      `b ≁ₜ readAction jj m0 (ISub anm e)`
         by simp[readAction_def, touches_def, expr_reads_def] >>
       metis_tac[apply_action_expr_eval_commutes, touches_SYM]) >>
   simp[dvread_def, DISJ_IMP_THM, FORALL_AND_THM, PULL_EXISTS] >>
-  qx_gen_tac `z` >> strip_tac >>
+  simp[PULL_FORALL] >> qx_gen_tac `z` >> rpt strip_tac >>
   qmatch_assum_rename_tac `w ≠ Variable v` [] >>
   `evalexpr m0 (VarExp v) = lookup_v m0 v ∧
    evalexpr m (VarExp v) = lookup_v m v`
     by simp[evalexpr_def] >>
-  `a ≁ₜ readAction jj m0 (VarExp v)`
+  `b ≁ₜ readAction jj m0 (VarExp v)`
     by simp[touches_def, readAction_def, expr_reads_def] >>
   metis_tac[apply_action_expr_eval_commutes, touches_SYM])
+
+val _ = temp_type_abbrev(
+  "tosty",
+  ``:(num list # memory #
+      (value list -> value, actionRW, num list)action_graph) option``)
 
 val graphOf_apply_action_diamond = store_thm(
   "graphOf_apply_action_diamond",
@@ -2030,9 +2069,9 @@ val graphOf_apply_action_diamond = store_thm(
       qmatch_assum_rename_tac `evalexpr m0 gd = Bool b` [] >>
       Cases_on `b` >> fs[] >> simp[PULL_EXISTS, EXISTS_PROD] >>
       qx_gen_tac `g'` >> rw[] >>
-      `i0 ∉ iterations g'`
+      `i0 ∉ idents g'`
         by metis_tac[ilistLT_stackInc, ilistLTE_trans,
-                     stackInc_EQ_NIL, ilistLE_REFL, graphOf_iterations_apart] >>
+                     stackInc_EQ_NIL, ilistLE_REFL, graphOf_idents_apart] >>
       fs[DISJ_IMP_THM, FORALL_AND_THM] >>
       `evalexpr m2 gd = evalexpr m0 gd ∧
        readAction i0 m2 gd = readAction i0 m0 gd`
@@ -2042,9 +2081,9 @@ val graphOf_apply_action_diamond = store_thm(
       ONCE_REWRITE_TAC [graphOf_def] >> simp[PULL_EXISTS, EXISTS_PROD] >>
       map_every qx_gen_tac [`i`, `m1`, `m2`, `a`, `dvs`, `g`] >> strip_tac >>
       fs[DISJ_IMP_THM, FORALL_AND_THM] >>
-      `i0 ∉ iterations g`
+      `i0 ∉ idents g`
         by metis_tac[ilistLT_stackInc, ilistLTE_trans,
-                     stackInc_EQ_NIL, ilistLE_REFL, graphOf_iterations_apart] >>
+                     stackInc_EQ_NIL, ilistLE_REFL, graphOf_idents_apart] >>
       `dvalues m2 d = dvalues m0 d ∧ domreadAction i0 m2 d = domreadAction i0 m0 d`
         by metis_tac[apply_action_dvalues_commutes] >>
       simp[] >> metis_tac[])
@@ -2057,11 +2096,11 @@ val graphOf_apply_action_diamond = store_thm(
       `∃m1'. graphOf i0 m2 c1 = SOME(i1,m1',g1) ∧
              apply_action a (SOME m0') = SOME m1'` by metis_tac[] >>
       simp[] >>
-      `i1 ≠ []` by metis_tac[graphOf_iterations_apart, LENGTH_NIL] >>
-      `∀b. b ∈ g2 ⇒ b.iter ∉ iterations g1`
+      `i1 ≠ []` by metis_tac[graphOf_idents_apart, LENGTH_NIL] >>
+      `∀b. b ∈ g2 ⇒ b.ident ∉ idents g1`
         by (gen_tac >> strip_tac >>
-            `b.iter ∈ iterations g2` by simp[iterations_thm] >>
-            metis_tac[graphOf_iterations_apart, ilistLTE_trans, ilistLE_REFL])>>
+            `b.ident ∈ idents g2` by simp[idents_thm] >>
+            metis_tac[graphOf_idents_apart, ilistLTE_trans, ilistLE_REFL])>>
       full_simp_tac (srw_ss() ++ CONJ_ss) [] >>
       metis_tac[])
   >- ((* parloop *)
@@ -2069,9 +2108,9 @@ val graphOf_apply_action_diamond = store_thm(
       ONCE_REWRITE_TAC [graphOf_def] >> simp[PULL_EXISTS, EXISTS_PROD] >>
       map_every qx_gen_tac [`i`, `m1`, `m2`, `a`, `dvs`, `g`] >> strip_tac >>
       fs[DISJ_IMP_THM, FORALL_AND_THM] >>
-      `i0 ∉ iterations g`
+      `i0 ∉ idents g`
         by metis_tac[ilistLT_stackInc, ilistLTE_trans,
-                     stackInc_EQ_NIL, ilistLE_REFL, graphOf_iterations_apart] >>
+                     stackInc_EQ_NIL, ilistLE_REFL, graphOf_idents_apart] >>
       `dvalues m2 d = dvalues m0 d ∧
        domreadAction i0 m2 d = domreadAction i0 m0 d`
         by metis_tac[apply_action_dvalues_commutes] >>
@@ -2080,25 +2119,23 @@ val graphOf_apply_action_diamond = store_thm(
       qx_gen_tac `cmds` >> strip_tac >> map_every qx_gen_tac [`i`, `m1`, `m2`, `a`, `g`] >>
       ONCE_REWRITE_TAC [graphOf_def] >>
       simp[OPT_SEQUENCE_EQ_SOME, combinTheory.o_ABS_R, MEM_MAPi, PULL_EXISTS] >>
-      qabbrev_tac `TOS = λt:(num list # memory #
-                                 (value, actionRW, num list)action_graph) option.
-                            THE (OPTION_MAP (SND o SND) t)` >> simp[] >>
+      qabbrev_tac `TOS = λt:tosty. THE (OPTION_MAP (SND o SND) t)` >> simp[] >>
       simp[FOLDR_MAPi, combinTheory.o_ABS_R] >> fs[] >> strip_tac >> fs[] >>
       csimp[] >>
       `∃m. pcg_eval g (SOME m2) = SOME m ∧ apply_action a (SOME m1) = SOME m`
         by metis_tac[pcg_eval_apply_action_diamond] >> simp[] >>
       qabbrev_tac `GG = λi. graphOf (i0 ++ [i;0])` >> simp[] >>
-      `∀it j. j < LENGTH cmds ∧ it ∈ iterations (TOS (GG j m0 (EL j cmds))) ⇒
+      `∀it j. j < LENGTH cmds ∧ it ∈ idents (TOS (GG j m0 (EL j cmds))) ⇒
               EL (LENGTH i0) it = j`
         by (rpt strip_tac >>
             `∃j' m' g'. graphOf (i0 ++ [j;0]) m0 (EL j cmds) = SOME (j',m',g')`
               by (fs[EXISTS_PROD] >> metis_tac[]) >>
             `TOS (GG j m0 (EL j cmds)) = g'` by simp[Abbr`GG`, Abbr`TOS`] >>
-            `∀k. k ∈ iterations g' ⇒
+            `∀k. k ∈ idents g' ⇒
                  LENGTH (i0 ++ [j;0]) ≤ LENGTH k ∧
                  TAKE (LENGTH (i0 ++ [j;0]) - 1) k = FRONT (i0 ++ [j;0])`
               by metis_tac[APPEND_eq_NIL, NOT_CONS_NIL,
-                           graphOf_iterations_apart] >>
+                           graphOf_idents_apart] >>
             lfs[FRONT_APPEND] >> pop_assum (qspec_then `it` mp_tac) >>
             simp[] >> strip_tac >>
             `EL (LENGTH i0) it = EL (LENGTH i0) (TAKE (LENGTH i0 + 1) it)`
@@ -2110,7 +2147,7 @@ val graphOf_apply_action_diamond = store_thm(
             simp[] >> simp[DISJOINT_DEF, EXTENSION] >> rpt strip_tac >>
             spose_not_then strip_assume_tac >>
             qmatch_assum_rename_tac
-              `iter ∈ iterations (TOS (GG i m0 (EL i cmds)))` [] >>
+              `ident ∈ idents (TOS (GG i m0 (EL i cmds)))` [] >>
             `i < LENGTH cmds ∧ i ≠ j` by decide_tac >> metis_tac[]) >>
       fs[PULL_EXISTS] >>
       `∀n. n < LENGTH cmds ⇒ ∃z. graphOf (i0 ++ [n;0]) m2 (EL n cmds) = SOME z`
@@ -2148,18 +2185,19 @@ val graphOf_apply_action_diamond = store_thm(
        evalexpr m2 i_e = evalexpr m0 i_e`
         by metis_tac[apply_action_expr_eval_commutes, touches_SYM] >>
       simp[] >>
-      `IS_SOME a.write ⇒ ¬MEM (THE a.write) rds`
-        by (Cases_on `a.write` >> fs[touches_def]) >>
+      `a.writes ≠ [] ⇒ ¬MEM (HD a.writes) rds`
+        by (Cases_on `a.writes` >> fs[touches_def] >> metis_tac[]) >>
       `getReads m2 ds = getReads m0 ds ∧
        dvreadAction (isuc i0) m2 ds = dvreadAction (isuc i0) m0 ds ∧
        MAP (evalDexpr m2) ds = MAP (evalDexpr m0) ds`
         by metis_tac[apply_action_dvreadAction_commutes] >> simp[] >>
-      qabbrev_tac `b = <| reads := []; write := SOME(Array anm iv);
-                          expr := K (opn rvs); iter := xx|>` >>
+      qabbrev_tac `b = <|
+        reads := []; writes := [Array anm iv]; ident := xx;
+        data := K (opn rvs) : value list -> value |>` >>
       `∀m. upd_array m anm iv (opn rvs) = apply_action b (SOME m)`
         by simp[apply_action_def, Abbr`b`, updf_def] >> fs[] >>
       `a ≁ₜ b` by (simp[touches_def, Abbr`b`] >> fs[touches_def] >>
-                  Cases_on `a.write` >> fs[]) >>
+                  Cases_on `a.writes` >> fs[]) >>
       metis_tac[successful_action_diamond])
   >- ((* assignvar *)
       simp[graphOf_def] >>
@@ -2171,8 +2209,10 @@ val graphOf_apply_action_diamond = store_thm(
        readAction jj m2 e = readAction jj m0 e`
         by metis_tac[apply_action_expr_eval_commutes] >>
       fs[readAction_def] >>
-      qabbrev_tac `b = <| reads := []; write := SOME (Variable vnm);
-                          expr := K (evalexpr m0 e); iter := jj |>` >>
+      qabbrev_tac `b = <|
+        reads := []; writes := [Variable vnm];
+        data := K (evalexpr m0 e) : value list -> value;
+        ident := jj |>` >>
       `∀m. updf (Variable vnm) (evalexpr m0 e) m = apply_action b (SOME m)`
         by simp[apply_action_def, Abbr`b`] >> fs[] >>
       `a ≁ₜ b` by (fs[Abbr`b`, touches_def] >> metis_tac[]) >>
@@ -2223,9 +2263,9 @@ val ITSET_gDELETE_ALL = store_thm(
 
 val pregreph_add_action_id = store_thm(
   "pregreph_add_action_id[simp]",
-  ``a.iter ∉ iterations g ⇒ pregraph a (a ⊕ g) = emptyG``,
+  ``a.ident ∉ idents g ⇒ pregraph a (a ⊕ g) = emptyG``,
   dsimp[pregraph_def, add_action_edges] >> csimp[] >> strip_tac >>
-  `a ∉ g` by (strip_tac >> fs[iterations_thm]) >>
+  `a ∉ g` by (strip_tac >> fs[idents_thm]) >>
   simp[] >>
   qmatch_abbrev_tac `ITSET (λb g. g \\ b) ss (a ⊕ g) = emptyG` >>
   `ss = ag_nodes (a ⊕ g)`
@@ -2255,24 +2295,24 @@ val pregraph_subset = store_thm(
   res_tac >> fs[]);
 
 val ITSET_DEL = prove(
-  ``∀s. FINITE s ⇒ ∀g a. a ∉ s ∧ a.iter ∉ iterations g ⇒
+  ``∀s. FINITE s ⇒ ∀g a. a ∉ s ∧ a.ident ∉ idents g ⇒
         ITSET (λb g. g \\ b) s (a ⊕ g) = a ⊕ ITSET (λb g. g \\ b) s g``,
   Induct_on `FINITE s` >>
   simp[ITSET_EMPTY, COMMUTING_ITSET_INSERT, gDELETE_commutes,
        DELETE_NON_ELEMENT_RWT] >>
   rpt strip_tac >>
-  `a.iter ∉ iterations (g \\ e)` by (fs[iterations_thm] >> metis_tac[]) >>
+  `a.ident ∉ idents (g \\ e)` by (fs[idents_thm] >> metis_tac[]) >>
   `(a ⊕ g) \\ e = a ⊕ (g \\ e)` suffices_by simp[] >>
   simp[graph_equality, add_action_edges, EQ_IMP_THM] >> rpt strip_tac >>
   simp[] >> metis_tac[]);
 
 val pregraph_add_action_1 = prove(
-  ``a.iter ∉ iterations g ∧ a ≠ b ∧ b ∈ g ∧ a ∼ₜ b ⇒
+  ``a.ident ∉ idents g ∧ a ≠ b ∧ b ∈ g ∧ a ∼ₜ b ⇒
     pregraph b (a ⊕ g) = a ⊕ pregraph b g``,
   simp[pregraph_def, add_action_edges] >> dsimp[] >> csimp[] >>
   strip_tac >>
   qmatch_abbrev_tac `ITSET del s1 (a ⊕ g) = a ⊕ ITSET del s2 g` >>
-  `a ∉ g` by (strip_tac >> fs[iterations_thm]) >>
+  `a ∉ g` by (strip_tac >> fs[idents_thm]) >>
   `s1 = s2`
     by dsimp[EXTENSION, Abbr`s1`, Abbr`s2`, EQ_IMP_THM] >>
   simp[Abbr`del`] >> `FINITE s2 ∧ a ∉ s2` suffices_by metis_tac[ITSET_DEL] >>
@@ -2282,10 +2322,10 @@ val pregraph_add_action_1 = prove(
   qunabbrev_tac `s2` >> fs[]);
 
 val pregraph_add_action_2 = prove(
-  ``a.iter ∉ iterations g ∧ a ≠ b ∧ b ∈ g ∧ a ≁ₜ b ⇒
+  ``a.ident ∉ idents g ∧ a ≠ b ∧ b ∈ g ∧ a ≁ₜ b ⇒
     pregraph b (a ⊕ g) = pregraph b g``,
   simp[pregraph_def, add_action_edges] >> rpt strip_tac >>
-  `a ∉ g` by (strip_tac >> fs[iterations_thm]) >>
+  `a ∉ g` by (strip_tac >> fs[idents_thm]) >>
   qmatch_abbrev_tac `ITSET del s1 (a ⊕ g) = ITSET del s2 g` >>
   `s1 = a INSERT s2`
     by (dsimp[EXTENSION, Abbr`s1`, Abbr`s2`, EQ_IMP_THM] >> csimp[] >>
@@ -2301,13 +2341,13 @@ val pregraph_add_action_2 = prove(
 
 val pregraph_add_action = store_thm(
   "pregraph_add_action",
-  ``a.iter ∉ iterations g ⇒
+  ``a.ident ∉ idents g ⇒
     pregraph b (a ⊕ g) =
       if b ∈ g then
         (if a ∼ₜ b then add_action a else I)
         (pregraph b g)
       else emptyG``,
-  strip_tac >> `a ∉ g` by (strip_tac >> fs[iterations_thm]) >>
+  strip_tac >> `a ∉ g` by (strip_tac >> fs[idents_thm]) >>
   rw[]
   >- (`a ≠ b` by (strip_tac >> fs[]) >>
       simp[pregraph_add_action_1])
@@ -2321,10 +2361,10 @@ val pregraph_add_postaction = store_thm(
   ``∀g a. a ∈ g ⇒ pregraph a (add_postaction b g) = pregraph a g``,
   ho_match_mp_tac graph_ind >> dsimp[] >> conj_tac
   >- (map_every qx_gen_tac [`a`, `g`] >> strip_tac >>
-      Cases_on `a.iter = b.iter` >- simp[add_postactionID] >>
+      Cases_on `a.ident = b.ident` >- simp[add_postactionID] >>
       simp[add_action_add_postaction_ASSOC]) >>
   map_every qx_gen_tac [`a`, `g`, `c`] >> rpt strip_tac >>
-  Cases_on `a.iter = b.iter` >- simp[add_postactionID] >>
+  Cases_on `a.ident = b.ident` >- simp[add_postactionID] >>
   simp[add_action_add_postaction_ASSOC, pregraph_add_action]);
 
 val pregraph_merge_graph = store_thm(
@@ -2342,8 +2382,8 @@ val pregraph_FOLDRi_merge_graph = store_thm(
       n < LENGTH list ∧ a ∈ f n (EL n list) ∧
       (∀i j. i < j ∧ j < LENGTH list ⇒
              ¬gtouches (f i (EL i list)) (f j (EL j list)) ∧
-             DISJOINT (iterations (f i (EL i list)))
-                      (iterations (f j (EL j list)))) ⇒
+             DISJOINT (idents (f i (EL i list)))
+                      (idents (f j (EL j list)))) ⇒
       pregraph a (FOLDRi (λn c. merge_graph (f n c)) emptyG list) =
       pregraph a (f n (EL n list))``,
   Induct >> dsimp[LT_SUC, combinTheory.o_ABS_L] >> conj_tac
@@ -2357,7 +2397,7 @@ val pregraph_FOLDRi_merge_graph = store_thm(
   `merge_graph g1 g2 = merge_graph g2 g1` suffices_by
     (disch_then SUBST1_TAC >> simp[pregraph_merge_graph]) >>
   match_mp_tac nontouching_merge_COMM >>
-  dsimp[iterations_FOLDRi_merge, Abbr`g2`] >>
+  dsimp[idents_FOLDRi_merge, Abbr`g2`] >>
   simp[gtouches_def, IN_FOLDRi_merge_graph] >>
   metis_tac[gtouches_def]);
 
@@ -2368,7 +2408,7 @@ val eval_graphOf_action = store_thm(
       m0 ≠ m ⇒
       ∀i0 i0' m0' g0.
         i0 ≠ [] ∧ graphOf i0 m0 c0 = SOME(i0', m0', g0) ⇒
-        ∃a. a ∈ g0 ∧ (∀b. b ∈ pregraph a g0 ⇒ b.write = NONE) ∧
+        ∃a. a ∈ g0 ∧ (∀b. b ∈ pregraph a g0 ⇒ b.writes = []) ∧
             apply_action a (SOME m0) = SOME m``,
   ho_match_mp_tac eval_ind' >> rpt conj_tac >> REWRITE_TAC []
   >- ((* head of Seq steps *)
@@ -2377,7 +2417,7 @@ val eval_graphOf_action = store_thm(
       simp[EXISTS_PROD, PULL_EXISTS] >>
       map_every qx_gen_tac [`ci`, `cm`, `cg`, `rg`] >>
       strip_tac >> rw[] >>
-      `∃a. a ∈ cg ∧ (∀b. b ∈ pregraph a cg ⇒ b.write = NONE) ∧
+      `∃a. a ∈ cg ∧ (∀b. b ∈ pregraph a cg ⇒ b.writes = []) ∧
            apply_action a (SOME m0) = SOME m`
         by metis_tac[] >>
       qexists_tac `a` >> simp[pregraph_merge_graph])
@@ -2399,8 +2439,7 @@ val eval_graphOf_action = store_thm(
       strip_tac >> fs[] >> simp[Once graphOf_def] >>
       simp[PULL_EXISTS, OPT_SEQUENCE_EQ_SOME, combinTheory.o_ABS_R] >>
       qabbrev_tac `
-        TOS = λt:(num list # memory #
-                  (value, actionRW, num list)action_graph) option.
+        TOS = λt:tosty.
                THE (OPTION_MAP (SND o SND) t)` >> simp[] >>
       map_every qx_gen_tac [`i0`, `m'`] >>
       qabbrev_tac `GG = λn. graphOf (i0 ++ [n;0])` >> simp[] >>
@@ -2413,16 +2452,16 @@ val eval_graphOf_action = store_thm(
       `∀x y z. TOS (SOME (x,y,z)) = z` by simp[Abbr`TOS`] >>
       lfs[] >>
       `∀i j. i < j ∧ j < LENGTH pfx + (LENGTH sfx + 1) ⇒
-             DISJOINT (iterations (gg i)) (iterations (gg j))`
+             DISJOINT (idents (gg i)) (idents (gg j))`
         by (map_every qx_gen_tac [`i`, `j`] >> strip_tac >>
             first_x_assum (fn th =>
               map_every (fn q => qspec_then q mp_tac th) [`i`, `j`]) >>
             simp[Abbr`GG`] >> rpt strip_tac >>
-            `(∀it. it ∈ iterations (gg i) ⇒
+            `(∀it. it ∈ idents (gg i) ⇒
                    TAKE (LENGTH (i0 ++ [i;0]) - 1) it = FRONT (i0 ++ [i;0])) ∧
-             (∀it. it ∈ iterations (gg j) ⇒
+             (∀it. it ∈ idents (gg j) ⇒
                    TAKE (LENGTH (i0 ++ [j;0]) - 1) it = FRONT (i0 ++ [j;0]))`
-              by metis_tac[graphOf_iterations_apart, APPEND_eq_NIL] >>
+              by metis_tac[graphOf_idents_apart, APPEND_eq_NIL] >>
             lfs[FRONT_APPEND] >> `i0 ++ [i] ≠ i0 ++ [j]` by simp[] >>
             simp[DISJOINT_DEF, EXTENSION] >> metis_tac[]) >>
       simp[IN_FOLDRi_merge_graph] >>
@@ -2468,23 +2507,23 @@ val GENLIST_CONG = store_thm(
 val _ = temp_overload_on ("MergeL", ``FOLDR merge_graph emptyG``)
 
 val FOLDR_merge_lemma = prove(
-  ``(∀g. MEM g l1 ⇒ ¬gtouches g e ∧ DISJOINT (iterations g) (iterations e)) ⇒
+  ``(∀g. MEM g l1 ⇒ ¬gtouches g e ∧ DISJOINT (idents g) (idents e)) ⇒
     FOLDR merge_graph emptyG (l1 ++ [e] ++ l2) =
     merge_graph e (FOLDR merge_graph emptyG (l1 ++ l2))``,
   Induct_on `l1` >> dsimp[merge_graph_ASSOC] >>
   metis_tac[nontouching_merge_COMM])
 
 val pcg_eval_merge_graph' = prove(
-  ``DISJOINT (iterations g1) (iterations g2) ⇒
+  ``DISJOINT (idents g1) (idents g2) ⇒
     pcg_eval (merge_graph g1 g2) = pcg_eval g2 o pcg_eval g1``,
   simp[FUN_EQ_THM] >> rpt strip_tac >>
   match_mp_tac pcg_eval_merge_graph >>
-  fs[DISJOINT_DEF, EXTENSION, iterations_thm] >>
+  fs[DISJOINT_DEF, EXTENSION, idents_thm] >>
   metis_tac[]);
 
-val iterations_MergeL = prove(
-  ``iterations (MergeL l) = BIGUNION (IMAGE iterations (set l))``,
-  dsimp[Once EXTENSION, iterations_FOLDR_merge_graph] >>
+val idents_MergeL = prove(
+  ``idents (MergeL l) = BIGUNION (IMAGE idents (set l))``,
+  dsimp[Once EXTENSION, idents_FOLDR_merge_graph] >>
   metis_tac[]);
 
 val MergeL_empty = prove(
@@ -2496,17 +2535,17 @@ val MergeL_append = prove(
   Induct_on `l1` >> simp[merge_graph_ASSOC])
 
 val imap_MergeL = prove(
-  ``(∀g. MEM g glist ⇒ INJ f (iterations g) UNIV) ∧
+  ``(∀g. MEM g glist ⇒ INJ f (idents g) UNIV) ∧
     (∀i j. i < j ∧ j < LENGTH glist ⇒
-           DISJOINT (iterations (EL i glist)) (iterations (EL j glist)) ∧
-           DISJOINT (IMAGE f (iterations (EL i glist)))
-                    (IMAGE f (iterations (EL j glist))))
+           DISJOINT (idents (EL i glist)) (idents (EL j glist)) ∧
+           DISJOINT (IMAGE f (idents (EL i glist)))
+                    (IMAGE f (idents (EL j glist))))
     ⇒
      imap f (MergeL glist) = MergeL (MAP (λg. imap f g) glist)``,
   Induct_on `glist` >> simp[] >> dsimp[LT_SUC] >> qx_gen_tac `h` >>
   strip_tac >> fs[] >>
-  `INJ f (iterations h ∪ iterations (MergeL glist)) UNIV`
-    by (simp[INJ_UNION_DOMAIN, iterations_MergeL] >>
+  `INJ f (idents h ∪ idents (MergeL glist)) UNIV`
+    by (simp[INJ_UNION_DOMAIN, idents_MergeL] >>
         dsimp[INJ_DEF] >> conj_tac
         >- (map_every qx_gen_tac [`it1`, `it2`, `g1`, `g2`] >> strip_tac >>
             Cases_on `g1 = g2` >- metis_tac [INJ_DEF] >>
@@ -2515,14 +2554,14 @@ val imap_MergeL = prove(
             `i ≠ j` by (strip_tac >> fs[]) >>
             fs[DISJOINT_DEF, EXTENSION] >>
             `i < j ∨ j < i` by decide_tac >> metis_tac[]) >>
-        `iterations h DIFF BIGUNION (IMAGE iterations (set glist)) =
-         iterations h`
+        `idents h DIFF BIGUNION (IMAGE idents (set glist)) =
+         idents h`
           by (simp[Once EXTENSION] >> qx_gen_tac `it` >> eq_tac >> simp[] >>
               strip_tac >> qx_gen_tac `s` >> Cases_on `it ∈ s` >> simp[] >>
               qx_gen_tac `g` >> disjneq_search >> BasicProvers.VAR_EQ_TAC >>
               fs[DISJOINT_DEF, EXTENSION] >> metis_tac[MEM_EL]) >>
-        `BIGUNION (IMAGE iterations (set glist)) DIFF iterations h =
-         BIGUNION (IMAGE iterations (set glist))`
+        `BIGUNION (IMAGE idents (set glist)) DIFF idents h =
+         BIGUNION (IMAGE idents (set glist))`
           by (simp[Once EXTENSION] >> dsimp[] >> qx_gen_tac `it` >>
               eq_tac >> strip_tac >- metis_tac[] >>
               fs[DISJOINT_DEF, EXTENSION] >> metis_tac[MEM_EL]) >>
@@ -2536,8 +2575,8 @@ val imap_MergeL = prove(
         `g ≠ h` by (strip_tac >> fs[DISJOINT_DEF, EXTENSION] >>
                     metis_tac[MEM_EL]) >>
         fs[DISJOINT_DEF, EXTENSION] >> metis_tac[MEM_EL]) >>
-  `DISJOINT (iterations h) (iterations (MergeL glist))`
-    by (simp[iterations_MergeL, DISJOINT_DEF, Once EXTENSION] >>
+  `DISJOINT (idents h) (idents (MergeL glist))`
+    by (simp[idents_MergeL, DISJOINT_DEF, Once EXTENSION] >>
         simp[GSYM IMP_DISJ_THM, PULL_FORALL] >>
         fs[DISJOINT_DEF, EXTENSION] >> metis_tac[MEM_EL]) >>
   simp[imap_merge_graph]);
@@ -2567,19 +2606,19 @@ val graphOf_correct_lemma = store_thm(
          by metis_tac[] >> simp[] >>
       qmatch_assum_rename_tac `
         graphOf i00 m00 (Seq rest) = SOME(i0',m0',rg)` []>>
-      `i00 ≠ [] ∧ i' ≠ []` by metis_tac[graphOf_iterations_apart, LENGTH_NIL] >>
+      `i00 ≠ [] ∧ i' ≠ []` by metis_tac[graphOf_idents_apart, LENGTH_NIL] >>
       `∃f. graphOf i' m00 (Seq rest) = SOME(f i0',m0',imap f rg) ∧
-           i' = f i00 ∧ INJ f (i0' INSERT iterations rg) UNIV`
+           i' = f i00 ∧ INJ f (i0' INSERT idents rg) UNIV`
         by metis_tac[graphOf_starting_id_irrelevant] >>
       simp[] >> fs[INJ_INSERT, IN_imap] >> dsimp[] >>
       dsimp[gtouches_def] >> rpt strip_tac
       >- (fs[gtouches_def] >> metis_tac[]) >>
       disj2_tac >>
-      `(∀j. j ∈ iterations rg ⇒ i00 ≤ j) ∧ ∀j. j ∈ iterations g00 ⇒ j < i00`
-        by metis_tac[graphOf_iterations_apart] >>
-      `∀a. a ∈ rg ⇒ a.iter ∉ iterations g00` suffices_by metis_tac[] >>
+      `(∀j. j ∈ idents rg ⇒ i00 ≤ j) ∧ ∀j. j ∈ idents g00 ⇒ j < i00`
+        by metis_tac[graphOf_idents_apart] >>
+      `∀a. a ∈ rg ⇒ a.ident ∉ idents g00` suffices_by metis_tac[] >>
       qx_gen_tac `a` >> strip_tac >>
-      `a.iter ∈ iterations rg` by simp[iterations_thm] >>
+      `a.ident ∈ idents rg` by simp[idents_thm] >>
       metis_tac[ilistLTE_trans, ilistLE_REFL])
   >- ((* seq head is Done *)
       simp[Once graphOf_def, SimpL ``$==>``] >>
@@ -2594,7 +2633,7 @@ val graphOf_correct_lemma = store_thm(
       strip_tac >>
       qmatch_assum_rename_tac `graphOf (stackInc i0) m0 cc = SOME (i,m,g)` []>>
       `∃f. graphOf i0 m0 cc = SOME (f i, m, imap f g) ∧
-           INJ f (i INSERT iterations g) UNIV ∧
+           INJ f (i INSERT idents g) UNIV ∧
            i0 = f (stackInc i0)`
         by metis_tac[graphOf_starting_id_irrelevant, stackInc_EQ_NIL] >>
       simp[])
@@ -2659,8 +2698,7 @@ val graphOf_correct_lemma = store_thm(
       simp[PULL_EXISTS, OPT_SEQUENCE_EQ_SOME, MEM_MAP, MEM_MAPi,
            combinTheory.o_ABS_R] >>
       qabbrev_tac `
-        TOS = λt:(num list # memory #
-                  (value, actionRW, num list)action_graph) option.
+        TOS = λt:tosty.
                THE (OPTION_MAP (SND o SND) t)` >> simp[] >>
       map_every qx_gen_tac [`i0`, `m00`] >>
       qabbrev_tac `GG = λn. graphOf (i0 ++ [n;0])` >> simp[] >>
@@ -2688,7 +2726,7 @@ val graphOf_correct_lemma = store_thm(
                 Cases_on `m = m0` >> simp[]
                 >- (first_x_assum (qspec_then `n` mp_tac) >>
                     simp[EL_APPEND1]) >>
-                `∃a. a ∈ gg ci ∧ (∀b. b ∈ pregraph a (gg ci) ⇒ b.write = NONE) ∧
+                `∃a. a ∈ gg ci ∧ (∀b. b ∈ pregraph a (gg ci) ⇒ b.writes = []) ∧
                      apply_action a (SOME m0) = SOME m`
                   by metis_tac[eval_graphOf_action, APPEND_eq_NIL] >>
                 first_x_assum (qspec_then `n` mp_tac) >> simp[EL_APPEND1] >>
@@ -2703,7 +2741,7 @@ val graphOf_correct_lemma = store_thm(
             Cases_on `m = m0` >> simp[]
             >- (first_x_assum (qspec_then `n` mp_tac) >>
                 simp[EL_APPEND1, EL_APPEND2]) >>
-            `∃a. a ∈ gg ci ∧ (∀b. b ∈ pregraph a (gg ci) ⇒ b.write = NONE) ∧
+            `∃a. a ∈ gg ci ∧ (∀b. b ∈ pregraph a (gg ci) ⇒ b.writes = []) ∧
                  apply_action a (SOME m0) = SOME m`
               by metis_tac[eval_graphOf_action, APPEND_eq_NIL] >>
             first_x_assum (qspec_then `n` mp_tac) >>
@@ -2756,8 +2794,8 @@ val graphOf_correct_lemma = store_thm(
       full_simp_tac (srw_ss() ++ ETA_ss) [] >>
       `∀g. MEM g (GENLIST gg ci) ⇒
            ¬gtouches g cg' ∧ ¬gtouches g (gg ci) ∧
-           DISJOINT (iterations g) (iterations cg') ∧
-           DISJOINT (iterations g) (iterations (gg ci))`
+           DISJOINT (idents g) (idents cg') ∧
+           DISJOINT (idents g) (idents (gg ci))`
         by (simp[MEM_GENLIST, PULL_EXISTS] >> qx_gen_tac `n` >>
             strip_tac >> conj_tac
             >- (first_x_assum (qspecl_then [`n`, `ci`] mp_tac) >>
@@ -2767,13 +2805,13 @@ val graphOf_correct_lemma = store_thm(
             `n < ci + (LENGTH sfx + 1)` by decide_tac >>
             pop_assum (fn th => first_x_assum (mp_tac o C MATCH_MP th)) >>
             simp[EL_APPEND1] >> qunabbrev_tac `GG` >> fs[] >> strip_tac >>
-            `(∀it. it ∈ iterations (gg n) ⇒
+            `(∀it. it ∈ idents (gg n) ⇒
                    TAKE (LENGTH (i0 ++ [n;0]) - 1) it =
                    FRONT (i0 ++ [n;0])) ∧
-             (∀it. it ∈ iterations cg' ∨ it ∈ iterations (gg ci) ⇒
+             (∀it. it ∈ idents cg' ∨ it ∈ idents (gg ci) ⇒
                    TAKE (LENGTH (i0 ++ [ci;0]) - 1) it =
                    FRONT (i0 ++ [ci;0]))`
-              by metis_tac[graphOf_iterations_apart, APPEND_eq_NIL] >>
+              by metis_tac[graphOf_idents_apart, APPEND_eq_NIL] >>
             fs[FRONT_APPEND] >> simp[DISJOINT_DEF, EXTENSION] >>
             `i0 ++ [ci] ≠ i0 ++ [n]` by simp[] >>
             metis_tac[]) >>
@@ -2782,29 +2820,29 @@ val graphOf_correct_lemma = store_thm(
       >- (qmatch_abbrev_tac `
             pcg_eval (merge_graph cg' RestG) (SOME m) = SOME m00
           ` >>
-          `DISJOINT (iterations cg') (iterations RestG) ∧
-           DISJOINT (iterations (gg ci)) (iterations RestG)`
+          `DISJOINT (idents cg') (idents RestG) ∧
+           DISJOINT (idents (gg ci)) (idents RestG)`
             suffices_by (strip_tac >> fs[pcg_eval_merge_graph']) >>
           ONCE_REWRITE_TAC [DISJOINT_SYM] >>
-          simp[Abbr`RestG`, iterations_MergeL, PULL_EXISTS] >>
+          simp[Abbr`RestG`, idents_MergeL, PULL_EXISTS] >>
           simp[MEM_GENLIST, PULL_EXISTS, PULL_FORALL] >>
           `∀n. n < LENGTH sfx ⇒
-               DISJOINT (iterations (gg (ci + (n + 1))))
-                        (iterations cg') ∧
-               DISJOINT (iterations (gg (ci + (n + 1))))
-                        (iterations (gg ci))`
+               DISJOINT (idents (gg (ci + (n + 1))))
+                        (idents cg') ∧
+               DISJOINT (idents (gg (ci + (n + 1))))
+                        (idents (gg ci))`
             suffices_by metis_tac[] >>
           gen_tac >> strip_tac >>
           `ci + (n + 1) < ci + (LENGTH sfx + 1)` by decide_tac >>
           pop_assum (fn th => first_x_assum (mp_tac o C MATCH_MP th)) >>
           simp[EL_APPEND2] >> qunabbrev_tac `GG` >> fs[] >> strip_tac >>
-          `(∀it. it ∈ iterations (gg (ci + (n + 1))) ⇒
+          `(∀it. it ∈ idents (gg (ci + (n + 1))) ⇒
                  TAKE (LENGTH (i0 ++ [ci + (n + 1);0]) - 1) it =
                  FRONT (i0 ++ [ci + (n + 1);0])) ∧
-           (∀it. it ∈ iterations cg' ∨ it ∈ iterations (gg ci) ⇒
+           (∀it. it ∈ idents cg' ∨ it ∈ idents (gg ci) ⇒
                  TAKE (LENGTH (i0 ++ [ci;0]) - 1) it =
                  FRONT (i0 ++ [ci;0]))`
-            by metis_tac[graphOf_iterations_apart, APPEND_eq_NIL] >>
+            by metis_tac[graphOf_idents_apart, APPEND_eq_NIL] >>
           fs[FRONT_APPEND] >>
           `i0 ++ [ci] ≠ i0 ++ [ci + (n + 1)]` by simp[] >>
           simp[DISJOINT_DEF, EXTENSION] >> metis_tac[]) >>
@@ -2815,10 +2853,10 @@ val graphOf_correct_lemma = store_thm(
       map_every qx_gen_tac [`g'`, `a1`, `a2`] >> strip_tac
       >- metis_tac[gtouches_def] >>
       map_every qexists_tac [`a1`, `a2`] >> simp[] >>
-      `a1.iter ∉ iterations (gg ci)` suffices_by simp[] >>
+      `a1.ident ∉ idents (gg ci)` suffices_by simp[] >>
       strip_tac >>
-      `a1.iter ∈ iterations BG` by simp[iterations_thm] >>
-      fs[iterations_FOLDR_merge_graph, Abbr`BG`]
+      `a1.ident ∈ idents BG` by simp[idents_thm] >>
+      fs[idents_FOLDR_merge_graph, Abbr`BG`]
       >- (res_tac >> fs[DISJOINT_DEF, EXTENSION] >>
           metis_tac[]) >>
       qpat_assum `MEM g (GENLIST f n)` mp_tac >>
@@ -2827,11 +2865,11 @@ val graphOf_correct_lemma = store_thm(
       `ci + (n + 1) < ci + (LENGTH sfx + 1)` by decide_tac >>
       pop_assum (fn th => first_x_assum (mp_tac o C MATCH_MP th)) >>
       simp[EL_APPEND2, Abbr`GG`] >> strip_tac >> fs[] >>
-      `TAKE (LENGTH (i0 ++ [ci; 0]) - 1) a1.iter =
+      `TAKE (LENGTH (i0 ++ [ci; 0]) - 1) a1.ident =
        FRONT (i0 ++ [ci;0]) ∧
-       TAKE (LENGTH (i0 ++ [ci + (n + 1); 0]) - 1) a1.iter =
+       TAKE (LENGTH (i0 ++ [ci + (n + 1); 0]) - 1) a1.ident =
        FRONT (i0 ++ [ci + (n + 1);0])`
-        by metis_tac[graphOf_iterations_apart, APPEND_eq_NIL] >>
+        by metis_tac[graphOf_idents_apart, APPEND_eq_NIL] >>
       fs[FRONT_APPEND])
   >- ((* par is all Dones component *)
       simp[graphOf_def, PULL_EXISTS, OPT_SEQUENCE_EQ_SOME,
